Regex/Compiler/Lemmas.lean
@@ -22,7 +22,7 @@ namespace Lemmas
 /-!
 ## Lemmas
 
-Proof that `Compiler.Code.compile` gives an array with the `Compiler.nextOfLt` and `NFA.Capture.valid` property
+Proof that `Compiler.Code.compile` gives an array with the `Compiler.NextOfLt` and `NFA.Capture.valid` property
 
 - `c_compile_spec`: main result
 -/
@@ -39,7 +39,7 @@ macro_rules | `(tactic|inst_mvar) => `(tactic| simp; (try and_intros; rfl); try 
 syntax "inst_mvars" : tactic
 macro_rules | `(tactic|inst_mvars) => `(tactic| simp; and_intros; all_goals try rfl)
 
-private theorem all_push {sid : Unchecked.State} (states : Array Unchecked.State)
+@[grind] private theorem all_push {sid : Unchecked.State} (states : Array Unchecked.State)
   (h : Unchecked.State.nextOf sid ≤ states.size)
   (hlt : ∀ (i : Nat) _, states[i].nextOf < states.size)
     : ∀ (i : Nat) _, ((states.push sid)[i].nextOf < (states.push sid).size) := by
@@ -84,42 +84,89 @@ instance {v : StateT σ Id α} {P : σ → Prop} {Q : α → σ → Prop}
   t.1 < r.size ∧ t.2 < r.size
 
 @[simp, grind] def statesNextOfLeLt (prevs : Array Unchecked.State) (s : Array Unchecked.State) :=
-  prevs.size ≤ s.size ∧ nextOfLt s
+  prevs.size ≤ s.size ∧ NextOfLt s
 
 @[simp, grind] def stateIdNextOfLt (prevs : Array Unchecked.State) (sid : Unchecked.StateID) (s : Array Unchecked.State) :=
-  prevs.size < s.size ∧ sid < s.size ∧ nextOfLt s
+  prevs.size < s.size ∧ sid < s.size ∧ NextOfLt s
 
 @[simp, grind] def stateIdNextOfLeLt (prevs : Array Unchecked.State) (sid : Unchecked.StateID) (s : Array Unchecked.State) :=
-  prevs.size ≤ s.size ∧ sid < s.size ∧ nextOfLt s
+  prevs.size ≤ s.size ∧ sid < s.size ∧ NextOfLt s
 
 @[simp, grind] def stateIdNextOfEqLt (prevs : Array Unchecked.State) (sid : Unchecked.StateID) (s : Array Unchecked.State) :=
-  prevs.size = s.size ∧ sid < s.size ∧ nextOfLt s
+  prevs.size = s.size ∧ sid < s.size ∧ NextOfLt s
 
 @[simp, grind] def tRefNextOfLt (prevs : Array Unchecked.State) (t : ThompsonRef) (s : Array Unchecked.State) :=
-  prevs.size < s.size ∧ tRefLt t s ∧ nextOfLt s
+  prevs.size < s.size ∧ tRefLt t s ∧ NextOfLt s
 
 @[simp, grind] def tRefNextOfLeLt (prevs : Array Unchecked.State) (t : ThompsonRef) (s : Array Unchecked.State) :=
-  prevs.size ≤ s.size ∧ tRefLt t s ∧ nextOfLt s
+  prevs.size ≤ s.size ∧ tRefLt t s ∧ NextOfLt s
 
-@[simp, grind] def cValid (caps : Array NFA.Capture) :=
-  NFA.Capture.valid caps
+def cValid (caps : Array NFA.Capture) :=
+  NFA.Capture.Valid caps
 
-@[simp, grind] def cMemAndValid (prev caps : Array NFA.Capture) :=
-  (∀ a ∈ prev, a ∈ caps) ∧ NFA.Capture.valid caps
+def cMemAndValid (prev caps : Array NFA.Capture) :=
+  (∀ a ∈ prev, a ∈ caps) ∧ NFA.Capture.Valid caps
 
-@[simp, grind] def cValidFunc (captures : Array NFA.Capture) : Array NFA.Capture → Prop :=
+def cValidFunc (captures : Array NFA.Capture) : Array NFA.Capture → Prop :=
     fun (curr : Array NFA.Capture) => curr = captures ∧ cValid captures
 
-@[simp] def cMemAndValidFunc (captures : Array NFA.Capture) : Array NFA.Capture → Prop :=
+def cMemAndValidFunc (captures : Array NFA.Capture) : Array NFA.Capture → Prop :=
     fun (curr : Array NFA.Capture) => curr = captures ∧ cMemAndValid captures curr
 
-@[simp] theorem cMemAndValid_of_cValid (captures : Array NFA.Capture)
+@[grind] theorem cap_exists_of_cap_role_end_of_cValid (caps : Array NFA.Capture) (h : cValid caps)
+  (a : NFA.Capture)  (h1 : a ∈ caps) (h2 : a.role = Capture.Role.End)
+    : ∃ (a' : NFA.Capture), a' ∈ caps ∧ a'.role = Capture.Role.Start ∧ a.group = a'.group := by
+  dsimp only [cValid] at h
+  have := Capture.Valid.forall h
+  simp_all
+
+@[grind] theorem cValid_of_empty (captures : Array NFA.Capture) (h : captures.size = 0)
+    : cValid captures := by
+  dsimp only [cValid]
+  apply Capture.Valid.mk
+  grind
+
+@[grind] theorem cValid_of_cMemAndValid (prevs caps : Array NFA.Capture)
+  (h : cMemAndValid prevs caps)
+    : cValid caps := by
+  dsimp [cMemAndValid] at h
+  grind [= cValid]
+
+@[simp] theorem cMemAndValid_of_cValid_of_eq (captures : Array NFA.Capture)
     : ∀ (s : Array NFA.Capture), s = captures ∧ cValid captures → cMemAndValid captures s := by
   intro s h
   unfold cValid at h
   unfold cMemAndValid
   rw [h.left]
   simp_all
+
+@[simp] theorem cMemAndValid_of_push_of_role_start (captures : Array NFA.Capture)
+  (capture : NFA.Capture) (hr : capture.role = Capture.Role.Start) (hc : cValid captures)
+    : cMemAndValid captures (captures.push capture) := by
+  simp [cMemAndValid]
+  simp [cValid] at hc
+  and_intros
+  · grind
+  · apply Capture.Valid.mk
+    intro c
+    have ⟨c', _⟩ := Capture.Valid.forall hc ⟨c, by grind⟩
+    exact ⟨c', by grind⟩
+
+@[grind] theorem cMemAndValid_of_push_of_role_end (captures : Array NFA.Capture)
+  (capture : NFA.Capture) (hc : cValid captures)
+  (h : ∃ c ∈ captures, c.role = Capture.Role.Start ∧ c.group = capture.group)
+    : cMemAndValid captures (captures.push capture) := by
+  simp [cMemAndValid]
+  simp [cValid] at hc
+  and_intros
+  · grind
+  · apply Capture.Valid.mk
+    intro c
+    cases Array.mem_or_eq_of_mem_push c.property.left
+    · have ⟨c', _⟩ := Capture.Valid.forall hc ⟨c, by grind⟩
+      exact ⟨c', by grind⟩
+    · have ⟨c', _⟩ := h
+      exact ⟨c', by grind⟩
 
 @[simp] theorem cMemAndValidFunc_of_cValidFunc (captures : Array NFA.Capture)
     : ∀ (s : Array NFA.Capture), cValidFunc captures s → cMemAndValidFunc captures s := by
@@ -176,41 +223,19 @@ theorem pure_of_imp_spec {x : α} {P1 P2 : α → σ → Prop} (h : ∀ a s, P1 
       (EStateM.pure x : EStateM ε σ α)
       ⦃post⟨fun r s => ⌜P2 r s⌝, fun _ => ⌜True⌝⟩⦄ := by
   simp [Triple, wp, EStateM.pure]
-  intro _ _
   grind
 
 @[spec] theorem patch_spec («from»: Unchecked.StateID) {«to» : Unchecked.StateID}
   {states : Array Unchecked.State}
-    : ⦃fun s => ⌜s = states ∧ nextOfLt states ∧ «from» < states.size ∧ «to» < states.size⌝⦄
+    : ⦃fun s => ⌜s = states ∧ NextOfLt states ∧ «from» < states.size ∧ «to» < states.size⌝⦄
       Code.patch «from» «to»
       ⦃post⟨fun _ r => ⌜stateIdNextOfEqLt states «to» r⌝, fun _ => ⌜True⌝ ⟩⦄ := by
-  mintro _
-  unfold Code.patch
-  mvcgen
-  all_goals simp_all <;> try intro _ _; expose_names
-  all_goals try (apply all_set_next_of_lt «from» _ states h_2.right.right.left ?_ (h.right.left)); try assumption
-  all_goals try simp_all [Unchecked.State.nextOf, h_2.right.right.right, Nat.max_lt]
-  all_goals try simp [wp]
-  all_goals try simp [nextOfLt] at h
-  expose_names
-  · simp [eat_lt «from» s_1 n (Unchecked.EatMode.Until s_1)
-      states (by grind) (by simp_all [Unchecked.EatMode.nextOf]) (by simp_all) (by grind)]
-  · simp [eat_lt «from» s_1 n (Unchecked.EatMode.Until s_1)
-      states (by grind) (by simp_all [Unchecked.EatMode.nextOf]) (by simp_all) (by grind)]
-  · simp [eat_lt «from» s_1 n (Unchecked.EatMode.ToLast 0)
-      states (by grind) (by simp_all [Unchecked.EatMode.nextOf]) (by simp_all) (by grind)]
-  · simp [eat_lt «from» s_1 n (Unchecked.EatMode.ToLast s_1)
-      states (by grind) (by simp_all [Unchecked.EatMode.nextOf]) (by simp_all) (by grind)]
-  · simp [change_frame_step_lt «from» f t states (by grind) (by simp_all) (by grind)]
-  · simp [change_frame_step_lt «from» f t states (by grind) (by simp_all) (by grind)]
-  · simp [binary_union_lt «from» alt1 alt2 states (by grind) (by simp_all) (by grind)]
-  · simp [binary_union_lt «from» alt1 alt2 states (by grind) (by simp_all) (by grind)]
-  · simp [union_lt «from» «to» alternates states (by simp_all) (by grind) (by grind) (by grind)]
-  · simp [union_reverse_lt «from» «to» alternates states (by simp_all) (by grind) (by grind) (by grind)]
+  mvcgen [Code.patch]
+  with grind
 
 @[spec] theorem patch_lift_spec («from»: Unchecked.StateID) {«to» : Unchecked.StateID}
   (states : Array Unchecked.State) (captures : Array NFA.Capture)
-    : ⦃fun s => ⌜(s.1 = states ∧ nextOfLt states ∧ «from» < states.size ∧ «to» < states.size)
+    : ⦃fun s => ⌜(s.1 = states ∧ NextOfLt states ∧ «from» < states.size ∧ «to» < states.size)
                  ∧ s.2.1 = captures ∧ cValid captures⌝⦄
       (Code.patch «from» «to» : Code.CompilerM Unit)
       ⦃post⟨fun _ s => ⌜stateIdNextOfEqLt states «to» s.1 ∧ s.2.1 = captures ∧ cMemAndValid captures s.2.1⌝,
@@ -218,21 +243,20 @@ theorem pure_of_imp_spec {x : α} {P1 P2 : α → σ → Prop} (h : ∀ a s, P1 
   exact coe_spec_EStateM_to_CompilerM (patch_spec _)
 
 @[spec] theorem push_spec (sid : Unchecked.State) (states : Array Unchecked.State)
-    : ⦃fun s => ⌜s = states ∧ nextOfLt states ∧ NFA.Unchecked.State.nextOf sid ≤ states.size⌝⦄
+    : ⦃fun s => ⌜s = states ∧ NextOfLt states ∧ NFA.Unchecked.State.nextOf sid ≤ states.size⌝⦄
       Code.push sid
       ⦃post⟨fun r s => ⌜stateIdNextOfLt states r s⌝⟩⦄ := by
   mvcgen [Code.push]
-  have := @all_push sid states (by simp_all) (by simp_all)
-  simp_all
+  with grind
 
 @[spec] theorem push_lift_spec (sid : Unchecked.State) (states : Array Unchecked.State)
-    : ⦃fun s => ⌜s = states ∧ nextOfLt states ∧ NFA.Unchecked.State.nextOf sid ≤ states.size⌝⦄
+    : ⦃fun s => ⌜s = states ∧ NextOfLt states ∧ NFA.Unchecked.State.nextOf sid ≤ states.size⌝⦄
       (Code.push sid : Code.PatchM Unchecked.StateID)
       ⦃post⟨fun r s => ⌜stateIdNextOfLt states r s⌝, fun _ => ⌜True⌝ ⟩⦄ := by
   exact ↑(push_spec sid states)
 
 @[spec] theorem push_run_spec (sid : Unchecked.State) (states : Array Unchecked.State)
-  (h1 : nextOfLt states) (h2 : NFA.Unchecked.State.nextOf sid ≤ states.size)
+  (h1 : NextOfLt states) (h2 : NFA.Unchecked.State.nextOf sid ≤ states.size)
     : ⦃⌜True⌝⦄
       ((Code.push sid).run states : Id (Unchecked.StateID × Array Unchecked.State))
       ⦃post⟨fun r => ⌜stateIdNextOfLt states r.1 r.2⌝⟩⦄ := by
@@ -247,7 +271,7 @@ theorem pure_of_imp_spec {x : α} {P1 P2 : α → σ → Prop} (h : ∀ a s, P1 
   and_intros <;> intros <;> simp_all <;> grind
 
 @[spec] theorem push_run_lift_spec (sid : Unchecked.State) (states : Array Unchecked.State)
-    : ⦃fun s => ⌜s.1 = states ∧ nextOfLt states ∧ NFA.Unchecked.State.nextOf sid ≤ states.size⌝⦄
+    : ⦃fun s => ⌜s.1 = states ∧ NextOfLt states ∧ NFA.Unchecked.State.nextOf sid ≤ states.size⌝⦄
       (Code.push sid states : Code.CompilerM (Unchecked.StateID × Array Unchecked.State))
       ⦃post⟨fun r _ => ⌜stateIdNextOfLt states r.1 r.2⌝, fun _ => ⌜True⌝ ⟩⦄ := by
   mvcgen
@@ -257,108 +281,106 @@ theorem pure_of_imp_spec {x : α} {P1 P2 : α → σ → Prop} (h : ∀ a s, P1 
   apply push_run_spec sid states <;> simp_all
 
 @[spec] theorem push'_spec (sid : Unchecked.State) (states : Array Unchecked.State)
-    : ⦃fun s => ⌜s = states ∧ nextOfLt states ∧ NFA.Unchecked.State.nextOf sid ≤ states.size⌝⦄
+    : ⦃fun s => ⌜s = states ∧ NextOfLt states ∧ NFA.Unchecked.State.nextOf sid ≤ states.size⌝⦄
       Code.push' sid
       ⦃post⟨fun r s => ⌜tRefNextOfLt states r s⌝⟩⦄ := by
   mvcgen [Code.push']
-  have := @all_push sid states (by simp_all) (by simp_all)
-  simp_all
+  with grind
 
 @[spec] theorem add_match_spec (pattern_id : PatternID) (states : Array Unchecked.State)
-    : ⦃fun s => ⌜s = states ∧ nextOfLt states⌝⦄
+    : ⦃fun s => ⌜s = states ∧ NextOfLt states⌝⦄
       Code.add_match pattern_id
       ⦃post⟨fun r s => ⌜stateIdNextOfLt states r s⌝⟩⦄ := by
   mvcgen [Code.add_match]
-  and_intros <;> simp_all [Unchecked.State.nextOf]
+  with grind
 
 @[spec] theorem add_match_lift_spec (pattern_id : PatternID) (states : Array Unchecked.State)
   (captures : Array NFA.Capture)
-    : ⦃fun s => ⌜(s.1 = states ∧ nextOfLt states) ∧ s.2.1 = captures ∧ cValid captures⌝⦄
+    : ⦃fun s => ⌜(s.1 = states ∧ NextOfLt states) ∧ s.2.1 = captures ∧ cValid captures⌝⦄
       (Code.add_match pattern_id : Code.CompilerM Unchecked.StateID)
       ⦃post⟨fun r s => ⌜stateIdNextOfLt states r s.1 ∧ s.2.1 = captures ∧ cMemAndValid captures s.2.1⌝ , fun _ => ⌜True⌝⟩⦄ := by
   exact coe_spec_StateT_to_CompilerM (add_match_spec _ _)
 
 @[spec] theorem add_union_spec (states : Array Unchecked.State)
-    : ⦃fun s => ⌜s = states ∧ nextOfLt states⌝⦄
+    : ⦃fun s => ⌜s = states ∧ NextOfLt states⌝⦄
       Code.add_union
       ⦃post⟨fun r s => ⌜stateIdNextOfLt states r s⌝⟩⦄ := by
   mvcgen [Code.add_union]
   and_intros <;> simp_all [Unchecked.State.nextOf, List.maxD]
 
 @[spec] theorem add_union_lift_spec (states : Array Unchecked.State)
-    : ⦃fun s => ⌜s = states ∧ nextOfLt states⌝⦄
+    : ⦃fun s => ⌜s = states ∧ NextOfLt states⌝⦄
       (Code.add_union : Code.PatchM Unchecked.StateID)
       ⦃post⟨fun r s => ⌜stateIdNextOfLt states r s⌝, fun _ => ⌜True⌝⟩⦄ := by
   exact ↑(add_union_spec states)
 
 @[spec] theorem add_union_lift'_spec (states : Array Unchecked.State) (captures : Array NFA.Capture)
-    : ⦃fun s => ⌜(s.1 = states ∧ nextOfLt states) ∧ s.2.1 = captures ∧ cValid captures⌝⦄
+    : ⦃fun s => ⌜(s.1 = states ∧ NextOfLt states) ∧ s.2.1 = captures ∧ cValid captures⌝⦄
       (Code.add_union : Code.CompilerM Unchecked.StateID)
       ⦃post⟨fun r s => ⌜stateIdNextOfLt states r s.1 ∧ s.2.1 = captures ∧ cMemAndValid captures s.2.1⌝, fun _ => ⌜True⌝⟩⦄ := by
   exact coe_spec_StateT_to_CompilerM (add_union_spec _)
 
 @[spec] theorem add_union_reverse_spec (states : Array Unchecked.State)
-    : ⦃fun s => ⌜s = states ∧ nextOfLt states⌝⦄
+    : ⦃fun s => ⌜s = states ∧ NextOfLt states⌝⦄
       Code.add_union_reverse
       ⦃post⟨fun r s => ⌜stateIdNextOfLt states r s⌝⟩⦄ := by
   mvcgen [Code.add_union_reverse]
   and_intros <;> simp_all [Unchecked.State.nextOf, List.maxD]
 
 @[spec] theorem add_union_reverse_lift_spec (states : Array Unchecked.State)
-    : ⦃fun s => ⌜s = states ∧ nextOfLt states⌝⦄
+    : ⦃fun s => ⌜s = states ∧ NextOfLt states⌝⦄
       (Code.add_union_reverse : Code.PatchM Unchecked.StateID)
       ⦃post⟨fun r s => ⌜stateIdNextOfLt states r s⌝, fun _ => ⌜True⌝⟩⦄ := by
   exact ↑(add_union_reverse_spec states)
 
 @[spec] theorem add_backrefence_spec (case_insensitive : Bool) (b : Nat) (states : Array Unchecked.State)
-    : ⦃fun s => ⌜s = states ∧ nextOfLt states⌝⦄
+    : ⦃fun s => ⌜s = states ∧ NextOfLt states⌝⦄
       Code.add_backrefence case_insensitive b
       ⦃post⟨fun r s => ⌜stateIdNextOfLt states r s⌝⟩⦄ := by
   mvcgen [Code.add_backrefence]
-  and_intros <;> simp_all [Unchecked.State.nextOf, List.maxD]
+  and_intros <;> grind
 
 @[spec] theorem add_backrefence_lift_spec (case_insensitive : Bool) (b : Nat) (states : Array Unchecked.State)
-    : ⦃fun s => ⌜s = states ∧ nextOfLt states⌝⦄
+    : ⦃fun s => ⌜s = states ∧ NextOfLt states⌝⦄
       (Code.add_backrefence case_insensitive b : (EStateM String (Array Unchecked.State) Unchecked.StateID))
       ⦃post⟨fun r s => ⌜stateIdNextOfLt states r s⌝, fun _ => ⌜True⌝⟩⦄ := by
   mvcgen [Code.add_backrefence]
 
 @[spec] theorem c_range_spec (start «end» : UInt32) (states : Array Unchecked.State)
-    : ⦃fun s => ⌜s = states ∧ nextOfLt states⌝⦄
+    : ⦃fun s => ⌜s = states ∧ NextOfLt states⌝⦄
       Code.c_range start «end»
       ⦃post⟨fun r s => ⌜tRefNextOfLt states r s⌝⟩⦄ := by
   mvcgen [Code.c_range]
-  and_intros <;> simp_all [Unchecked.State.nextOf]
-  grind
+  with grind
 
 @[spec] theorem add_empty_spec (states : Array Unchecked.State)
-    : ⦃fun s => ⌜s = states ∧ nextOfLt states⌝⦄
+    : ⦃fun s => ⌜s = states ∧ NextOfLt states⌝⦄
       Code.add_empty
       ⦃post⟨fun r s => ⌜stateIdNextOfLt states r s⌝⟩⦄ := by
   mvcgen [Code.add_empty]
-  and_intros <;> simp_all [Unchecked.State.nextOf, List.maxD]
+  with grind
 
 @[spec] theorem add_empty_lift_spec (states : Array Unchecked.State)
-    : ⦃fun s => ⌜s = states ∧ nextOfLt states⌝⦄
+    : ⦃fun s => ⌜s = states ∧ NextOfLt states⌝⦄
       (Code.add_empty : Code.PatchM Unchecked.StateID)
       ⦃post⟨fun r s => ⌜stateIdNextOfLt states r s⌝, fun _ => ⌜True⌝⟩⦄ := by
   exact ↑(add_empty_spec states)
 
 theorem add_empty_lift'_spec (states : Array Unchecked.State) (captures : Array NFA.Capture)
-    : ⦃fun s => ⌜(s.1 = states ∧ nextOfLt states) ∧ s.2.1 = captures ∧ cValid captures⌝⦄
+    : ⦃fun s => ⌜(s.1 = states ∧ NextOfLt states) ∧ s.2.1 = captures ∧ cValid captures⌝⦄
       (Code.add_empty : Code.CompilerM Unchecked.StateID)
       ⦃post⟨fun r s => ⌜stateIdNextOfLt states r s.1 ∧ s.2.1 = captures ∧ cMemAndValid captures s.2.1⌝, fun _ => ⌜True⌝⟩⦄ := by
   exact coe_spec_StateT_to_CompilerM (add_empty_spec _)
 
 @[spec] theorem add_fail_spec (states : Array Unchecked.State)
-    : ⦃fun s => ⌜s = states ∧ nextOfLt states⌝⦄
+    : ⦃fun s => ⌜s = states ∧ NextOfLt states⌝⦄
       Code.add_fail
       ⦃post⟨fun r s => ⌜stateIdNextOfLt states r s⌝⟩⦄ := by
   mvcgen [Code.add_fail]
-  and_intros <;> simp_all [Unchecked.State.nextOf, List.maxD]
+  with grind
 
 @[spec] theorem add_fail_lift_spec (states : Array Unchecked.State)
-    : ⦃fun s => ⌜s = states ∧ nextOfLt states⌝⦄
+    : ⦃fun s => ⌜s = states ∧ NextOfLt states⌝⦄
       (Code.add_fail : Code.PatchM Unchecked.StateID)
       ⦃post⟨fun r s => ⌜stateIdNextOfLt states r s⌝, fun _ => ⌜True⌝⟩⦄ := by
   exact ↑(add_fail_spec states)
@@ -375,55 +397,55 @@ theorem eat_next_of_le (states : Array Unchecked.State) (h : mode.nextOf < state
     <;> exact And.intro (by grind) (by exact Nat.zero_le states.size)
 
 @[spec] theorem add_eat_spec (mode : Unchecked.EatMode) (states : Array Unchecked.State)
-    : ⦃fun s => ⌜s = states ∧ nextOfLt states ∧ (mode.nextOf < states.size)⌝⦄
+    : ⦃fun s => ⌜s = states ∧ NextOfLt states ∧ (mode.nextOf < states.size)⌝⦄
       Code.add_eat mode
       ⦃post⟨fun r s => ⌜stateIdNextOfLt states r s⌝⟩⦄ := by
   mvcgen [Code.add_eat]
   simp_all [@eat_next_of_le mode states (by simp_all)]
 
 @[spec] theorem add_change_state_spec (states : Array Unchecked.State)
-    : ⦃fun s => ⌜s = states ∧ nextOfLt states⌝⦄
+    : ⦃fun s => ⌜s = states ∧ NextOfLt states⌝⦄
       Code.add_change_state
       ⦃post⟨fun r s => ⌜stateIdNextOfLt states r s⌝⟩⦄ := by
   mvcgen [Code.add_change_state]
-  and_intros <;> simp_all [Unchecked.State.nextOf, List.maxD]
+  with grind
 
 @[spec] theorem add_change_state_lift_spec (states : Array Unchecked.State)
-    : ⦃fun s => ⌜s = states ∧ nextOfLt states⌝⦄
+    : ⦃fun s => ⌜s = states ∧ NextOfLt states⌝⦄
       (Code.add_change_state : Code.PatchM Unchecked.StateID)
       ⦃post⟨fun r s => ⌜stateIdNextOfLt states r s⌝, fun _ => ⌜True⌝⟩⦄ := by
   exact ↑(add_change_state_spec states)
 
 @[spec] theorem add_remove_state_spec (states : Array Unchecked.State)
-    : ⦃fun s => ⌜s = states ∧ nextOfLt states⌝⦄
+    : ⦃fun s => ⌜s = states ∧ NextOfLt states⌝⦄
       Code.add_remove_state
       ⦃post⟨fun r s => ⌜stateIdNextOfLt states r s⌝⟩⦄ := by
   mvcgen [Code.add_remove_state]
-  and_intros <;> simp_all [Unchecked.State.nextOf, List.maxD]
+  with grind
 
 @[spec] theorem add_next_char_spec (offset : Nat) (states : Array Unchecked.State)
-    : ⦃fun s => ⌜s = states ∧ nextOfLt states⌝⦄
+    : ⦃fun s => ⌜s = states ∧ NextOfLt states⌝⦄
       Code.add_next_char offset
       ⦃post⟨fun r s => ⌜stateIdNextOfLt states r s⌝⟩⦄ := by
   mvcgen [Code.add_next_char]
-  and_intros <;> simp_all [Unchecked.State.nextOf, List.maxD]
+  with grind
 
 @[spec] theorem add_next_char_lift_spec (offset : Nat) (states : Array Unchecked.State)
   (captures : Array NFA.Capture)
-    : ⦃fun s => ⌜(s.1 = states ∧ nextOfLt states) ∧ s.2.1 = captures ∧ cValid captures⌝⦄
+    : ⦃fun s => ⌜(s.1 = states ∧ NextOfLt states) ∧ s.2.1 = captures ∧ cValid captures⌝⦄
       (Code.add_next_char offset : Code.CompilerM Unchecked.StateID)
       ⦃post⟨fun r s => ⌜stateIdNextOfLt states r s.1 ∧ s.2.1 = captures ∧ cMemAndValid captures s.2.1⌝, fun _ => ⌜True⌝⟩⦄ := by
   exact coe_spec_StateT_to_CompilerM (add_next_char_spec _ _)
 
 @[spec] theorem c_empty_spec (states : Array Unchecked.State)
-    : ⦃fun s => ⌜s = states ∧ nextOfLt states⌝⦄
+    : ⦃fun s => ⌜s = states ∧ NextOfLt states⌝⦄
       Code.c_empty
       ⦃post⟨fun r s => ⌜tRefNextOfLt states r s⌝⟩⦄ := by
   mvcgen [Code.c_empty]
-  and_intros <;> simp_all [Unchecked.State.nextOf]
+  with grind
 
 @[spec] theorem c_empty_lift_spec (states : Array Unchecked.State) (captures : Array NFA.Capture)
-    : ⦃fun s => ⌜(s.1 = states ∧ nextOfLt states) ∧ s.2.1 = captures ∧ cValid captures⌝⦄
+    : ⦃fun s => ⌜(s.1 = states ∧ NextOfLt states) ∧ s.2.1 = captures ∧ cValid captures⌝⦄
       (Code.c_empty : Code.CompilerM ThompsonRef)
       ⦃post⟨fun r s => ⌜tRefNextOfLt states r s.1 ∧ s.2.1 = captures ∧ cMemAndValid captures s.2.1⌝, fun _ => ⌜True⌝⟩⦄ := by
   exact coe_spec_StateT_to_CompilerM (c_empty_spec _)
@@ -441,63 +463,64 @@ theorem eat_next_of_le (states : Array Unchecked.State) (h : mode.nextOf < state
   exact List.maxD_of_all_map_le h
 
 @[spec] theorem add_sparse_spec (trans : Array Unchecked.Transition) (states : Array Unchecked.State)
-    : ⦃fun s => ⌜s = states ∧ nextOfLt states ∧ ∀ (i : Nat) _, trans[i].next ≤ states.size⌝⦄
+    : ⦃fun s => ⌜s = states ∧ NextOfLt states ∧ ∀ (i : Nat) _, trans[i].next ≤ states.size⌝⦄
       Code.add_sparse trans
       ⦃post⟨fun r s => ⌜stateIdNextOfLt states r s⌝⟩⦄ := by
   mvcgen [Code.add_sparse]
   and_intros <;> simp_all
 
 @[spec] theorem c_unicode_class_spec (cls : ClassUnicode) (states : Array Unchecked.State)
-    : ⦃fun s => ⌜s = states ∧ nextOfLt states⌝⦄
+    : ⦃fun s => ⌜s = states ∧ NextOfLt states⌝⦄
       Code.c_unicode_class cls
       ⦃post⟨fun r s => ⌜tRefNextOfLt states r s⌝⟩⦄ := by
   mvcgen [Code.c_unicode_class]
-  all_goals simp_all; grind
+  with grind
 
 @[spec] theorem c_unicode_class_lift_spec (cls : ClassUnicode) (states : Array Unchecked.State)
   (captures : Array NFA.Capture)
-    : ⦃fun s => ⌜(s.1 = states ∧ nextOfLt states) ∧ s.2.1 = captures ∧ cValid captures⌝⦄
+    : ⦃fun s => ⌜(s.1 = states ∧ NextOfLt states) ∧ s.2.1 = captures ∧ cValid captures⌝⦄
       (Code.c_unicode_class cls : Code.CompilerM ThompsonRef)
       ⦃post⟨fun r s => ⌜tRefNextOfLt states r s.1 ∧ s.2.1 = captures ∧ cMemAndValid captures s.2.1⌝, fun _ => ⌜True⌝⟩⦄ := by
   exact coe_spec_StateT_to_CompilerM (c_unicode_class_spec _ _)
 
 @[spec] theorem c_literal_spec (c : Char) (states : Array Unchecked.State)
-    : ⦃fun s => ⌜s = states ∧ nextOfLt states⌝⦄
+    : ⦃fun s => ⌜s = states ∧ NextOfLt states⌝⦄
       Code.c_literal c
       ⦃post⟨fun r s => ⌜tRefNextOfLt states r s⌝⟩⦄ := by
   mvcgen [Code.c_literal]
 
 @[spec] theorem c_literal_lift_spec (c : Char) (states : Array Unchecked.State)
   (captures : Array NFA.Capture)
-    : ⦃fun s => ⌜(s.1 = states ∧ nextOfLt states) ∧ s.2.1 = captures ∧ cValid captures⌝⦄
+    : ⦃fun s => ⌜(s.1 = states ∧ NextOfLt states) ∧ s.2.1 = captures ∧ cValid captures⌝⦄
       (Code.c_literal c : Code.CompilerM ThompsonRef)
       ⦃post⟨fun r s => ⌜tRefNextOfLt states r s.1 ∧ s.2.1 = captures ∧ cMemAndValid captures s.2.1⌝, fun _ => ⌜True⌝⟩⦄ := by
   exact coe_spec_StateT_to_CompilerM (c_literal_spec _ _)
 
 @[spec] theorem c_look_spec (look : Syntax.Look) (states : Array Unchecked.State)
-    : ⦃fun s => ⌜s = states ∧ nextOfLt states⌝⦄
+    : ⦃fun s => ⌜s = states ∧ NextOfLt states⌝⦄
       Code.c_look look
       ⦃post⟨fun r s => ⌜tRefNextOfLt states r s⌝ ⟩⦄ := by
-  mvcgen [Code.c_look] <;> simp_all [Unchecked.State.nextOf]
+  mvcgen [Code.c_look]
+  with grind
 
 @[spec] theorem c_look_lift_spec (look : Syntax.Look) (states : Array Unchecked.State)
   (captures : Array NFA.Capture)
-    : ⦃fun s => ⌜(s.1 = states ∧ nextOfLt states) ∧ s.2.1 = captures ∧ cValid captures⌝⦄
+    : ⦃fun s => ⌜(s.1 = states ∧ NextOfLt states) ∧ s.2.1 = captures ∧ cValid captures⌝⦄
       (Code.c_look look : Code.CompilerM ThompsonRef)
       ⦃post⟨fun r s => ⌜tRefNextOfLt states r s.1 ∧ s.2.1 = captures ∧ cMemAndValid captures s.2.1⌝, fun _ => ⌜True⌝⟩⦄ := by
   exact coe_spec_StateT_to_CompilerM (c_look_spec _ _)
 
 @[spec] theorem c_possessive_spec (tref : ThompsonRef) (states : Array Unchecked.State)
     : ⦃fun s => ⌜s = states ∧ tref.start < states.size
-                      ∧ tref.end < states.size ∧ nextOfLt states⌝⦄
+                      ∧ tref.end < states.size ∧ NextOfLt states⌝⦄
       Code.c_possessive tref
       ⦃post⟨fun r s => ⌜tRefNextOfLt states r s⌝, fun _ => ⌜True⌝⟩⦄ := by
   mvcgen [Code.c_possessive]
-  all_goals simp_all [Unchecked.EatMode.nextOf] <;> grind
+  with grind
 
 @[spec] theorem c_possessive_lift_spec (tref : ThompsonRef) (states : Array Unchecked.State)
   (captures : Array NFA.Capture)
-    : ⦃fun s => ⌜(s.1 = states ∧ tref.start < states.size ∧ tref.end < states.size ∧ nextOfLt states)
+    : ⦃fun s => ⌜(s.1 = states ∧ tref.start < states.size ∧ tref.end < states.size ∧ NextOfLt states)
                   ∧ s.2.1 = captures ∧ cValid captures⌝⦄
       (Code.c_possessive tref : Code.CompilerM ThompsonRef)
       ⦃post⟨fun r s => ⌜tRefNextOfLt states r s.1 ∧ s.2.1 = captures ∧ cMemAndValid captures s.2.1⌝, fun _ => ⌜True⌝⟩⦄ := by
@@ -514,178 +537,167 @@ theorem tref_le_of_lt_spec (states : Array Unchecked.State)
 -- relax postcondition of c_possessive_lift_spec
 theorem c_possessive_le_lift_spec (tref : ThompsonRef) (states : Array Unchecked.State)
   (captures : Array NFA.Capture)
-    : ⦃fun s => ⌜(s.1 = states ∧ tref.start < states.size ∧ tref.end < states.size ∧ nextOfLt states)
+    : ⦃fun s => ⌜(s.1 = states ∧ tref.start < states.size ∧ tref.end < states.size ∧ NextOfLt states)
                 ∧ s.2.1 = captures ∧ cValid captures⌝⦄
       (Code.c_possessive tref : Code.CompilerM ThompsonRef)
       ⦃post⟨fun r s => ⌜tRefNextOfLeLt states r s.1 ∧ s.2.1 = captures ∧ cMemAndValid captures s.2.1⌝, fun _ => ⌜True⌝⟩⦄ := by
   have := Triple.bind _ _ (c_possessive_lift_spec tref states captures) (tref_le_of_lt_spec states)
   rwa [lift_CompilerM_bind_pure (Code.c_possessive tref)] at this
 
-@[spec] theorem c_cap'_start_spec (group slot: Nat)
-  (isValid : Capture.IsValid Capture.Role.Start group slot) (states : Array Unchecked.State)
+@[spec] theorem c_cap'_start_spec (group : Nat) (states : Array Unchecked.State)
   (captures : Array NFA.Capture)
-    : ⦃fun s => ⌜s.1 = states ∧ nextOfLt states ∧ s.2.1 = captures ∧ cValid captures⌝⦄
-      Code.c_cap' Capture.Role.Start group slot isValid
+    : ⦃fun s => ⌜s.1 = states ∧ NextOfLt states ∧ s.2.1 = captures ∧ cValid captures⌝⦄
+      Code.c_cap' Capture.Role.Start group
       ⦃post⟨fun r s => ⌜stateIdNextOfLt states r s.1
                         ∧ cMemAndValid captures s.2.1
-                        ∧ (NFA.Capture.mk Capture.Role.Start group slot isValid) ∈ s.2.1⌝, fun _ => ⌜True⌝⟩⦄ := by
-  mvcgen [Code.c_cap'] <;> simp_all [Unchecked.State.nextOf]
-  intros
-  and_intros
-  · intros
-    and_intros <;> have := isValid <;> simp_all <;> grind
-  · intros
-    and_intros
-    · rename_i h _ _ _
-      cases h; have := isValid; simp_all; grind
-    · have := isValid; simp_all; grind
-  · grind
+                        ∧ (NFA.Capture.mk Capture.Role.Start group) ∈ s.2.1⌝, fun _ => ⌜True⌝⟩⦄ := by
+  mvcgen [Code.c_cap']
+  with grind
+  simp_all
 
-@[spec] theorem c_cap'_end_spec (group slot: Nat)
-  (isValid : Capture.IsValid Capture.Role.End group slot) (states : Array Unchecked.State)
+@[spec] theorem c_cap'_end_spec (group : Nat) (states : Array Unchecked.State)
   (captures : Array NFA.Capture) (h : ∃ c ∈ captures, c.role = Capture.Role.Start ∧ c.group = group)
-    : ⦃fun s => ⌜s.1 = states ∧ nextOfLt states ∧ s.2.1 = captures ∧ cValid captures⌝⦄
-      Code.c_cap' Capture.Role.End group slot isValid
+    : ⦃fun s => ⌜s.1 = states ∧ NextOfLt states ∧ s.2.1 = captures ∧ cValid captures⌝⦄
+      Code.c_cap' Capture.Role.End group
       ⦃post⟨fun r s => ⌜stateIdNextOfLt states r s.1 ∧ cMemAndValid captures s.2.1⌝, fun _ => ⌜True⌝⟩⦄ := by
-  mvcgen [Code.c_cap'] <;> simp_all [Unchecked.State.nextOf]
-  intros
-  and_intros <;> have := isValid <;> simp_all <;> grind
+  mvcgen [Code.c_cap']
+  with grind
 
 @[spec] theorem c_back_ref_spec (case_insensitive : Bool) (n : Nat)  (states : Array Unchecked.State)
-    : ⦃fun s => ⌜s = states ∧ nextOfLt states⌝⦄
+    : ⦃fun s => ⌜s = states ∧ NextOfLt states⌝⦄
       Code.c_back_ref case_insensitive n
       ⦃post⟨fun r s => ⌜tRefNextOfLt states r s⌝, fun _ => ⌜True⌝⟩⦄ := by
   mvcgen [Code.c_back_ref]
-  all_goals grind
+  with grind
 
 @[spec] theorem c_back_ref_lift_spec (case_insensitive : Bool) (n : Nat)  (states : Array Unchecked.State)
   (captures : Array NFA.Capture)
-    : ⦃fun s => ⌜(s.1 = states ∧ nextOfLt states) ∧ s.2.1 = captures ∧ cValid captures⌝⦄
+    : ⦃fun s => ⌜(s.1 = states ∧ NextOfLt states) ∧ s.2.1 = captures ∧ cValid captures⌝⦄
       (Code.c_back_ref case_insensitive n : Code.CompilerM ThompsonRef)
       ⦃post⟨fun r s => ⌜tRefNextOfLt states r s.1 ∧ s.2.1 = captures ∧ cMemAndValid captures s.2.1⌝, fun _ => ⌜True⌝⟩⦄ := by
   exact coe_spec_EStateM_to_CompilerM (c_back_ref_spec _ _ _)
 
 @[spec] theorem c_lookaround_PositiveLookahead_spec (compiled : ThompsonRef) (states : Array Unchecked.State)
-    : ⦃fun s => ⌜s = states ∧ tRefLt compiled states ∧ nextOfLt states⌝⦄
+    : ⦃fun s => ⌜s = states ∧ tRefLt compiled states ∧ NextOfLt states⌝⦄
       Code.c_lookaround_PositiveLookahead compiled
       ⦃post⟨fun r s => ⌜tRefNextOfLeLt states r s⌝, fun _ => ⌜True⌝⟩⦄ := by
   mvcgen [Code.c_lookaround_PositiveLookahead]
-  all_goals grind
+  with grind
 
 @[spec] theorem c_lookaround_PositiveLookahead_lift_spec (compiled : ThompsonRef) (states : Array Unchecked.State)
   (captures : Array NFA.Capture)
-    : ⦃fun s => ⌜(s.1 = states ∧ tRefLt compiled states ∧ nextOfLt states)
+    : ⦃fun s => ⌜(s.1 = states ∧ tRefLt compiled states ∧ NextOfLt states)
                   ∧ s.2.1 = captures ∧ cValid captures⌝⦄
       (Code.c_lookaround_PositiveLookahead compiled : Code.CompilerM ThompsonRef)
       ⦃post⟨fun r s => ⌜tRefNextOfLeLt states r s.1 ∧ s.2.1 = captures ∧ cMemAndValid captures s.2.1⌝, fun _ => ⌜True⌝⟩⦄ := by
   exact coe_spec_EStateM_to_CompilerM (c_lookaround_PositiveLookahead_spec _ _)
 
 @[spec] theorem c_lookaround_NegativeLookahead_spec (compiled : ThompsonRef) (states : Array Unchecked.State)
-    : ⦃fun s => ⌜s = states ∧ tRefLt compiled states ∧ nextOfLt states⌝⦄
+    : ⦃fun s => ⌜s = states ∧ tRefLt compiled states ∧ NextOfLt states⌝⦄
       Code.c_lookaround_NegativeLookahead compiled
       ⦃post⟨fun r s => ⌜tRefNextOfLeLt states r s⌝, fun _ => ⌜True⌝⟩⦄ := by
   mvcgen [Code.c_lookaround_NegativeLookahead]
-  all_goals grind
+  with grind
 
 @[spec] theorem c_lookaround_NegativeLookahead_lift_spec (compiled : ThompsonRef) (states : Array Unchecked.State)
   (captures : Array NFA.Capture)
-    : ⦃fun s => ⌜(s.1 = states ∧ tRefLt compiled states ∧ nextOfLt states)
+    : ⦃fun s => ⌜(s.1 = states ∧ tRefLt compiled states ∧ NextOfLt states)
                   ∧ s.2.1 = captures ∧ cValid captures⌝⦄
       (Code.c_lookaround_NegativeLookahead compiled : Code.CompilerM ThompsonRef)
       ⦃post⟨fun r s => ⌜tRefNextOfLeLt states r s.1 ∧ s.2.1 = captures ∧ cMemAndValid captures s.2.1⌝, fun _ => ⌜True⌝⟩⦄ := by
   exact coe_spec_EStateM_to_CompilerM (c_lookaround_NegativeLookahead_spec _ _)
 
 @[spec] theorem c_lookaround_PositiveLookbehind_spec (next_char : Unchecked.StateID) (compiled : ThompsonRef) (states : Array Unchecked.State)
-    : ⦃fun s => ⌜s = states ∧ next_char < states.size ∧ tRefLt compiled states ∧ nextOfLt states⌝⦄
+    : ⦃fun s => ⌜s = states ∧ next_char < states.size ∧ tRefLt compiled states ∧ NextOfLt states⌝⦄
       Code.c_lookaround_PositiveLookbehind next_char compiled
       ⦃post⟨fun r s => ⌜tRefNextOfLeLt states r s⌝, fun _ => ⌜True⌝⟩⦄ := by
   mvcgen [Code.c_lookaround_PositiveLookbehind]
-  all_goals grind
+  with grind
 
 @[spec] theorem c_lookaround_PositiveLookbehind_lift_spec (next_char : Unchecked.StateID) (compiled : ThompsonRef) (states : Array Unchecked.State)
   (captures : Array NFA.Capture)
-    : ⦃fun s => ⌜(s.1 = states ∧ next_char < states.size ∧ tRefLt compiled states ∧ nextOfLt states)
+    : ⦃fun s => ⌜(s.1 = states ∧ next_char < states.size ∧ tRefLt compiled states ∧ NextOfLt states)
                   ∧ s.2.1 = captures ∧ cValid captures⌝⦄
       (Code.c_lookaround_PositiveLookbehind next_char compiled : Code.CompilerM ThompsonRef)
       ⦃post⟨fun r s => ⌜tRefNextOfLeLt states r s.1 ∧ s.2.1 = captures ∧ cMemAndValid captures s.2.1⌝, fun _ => ⌜True⌝⟩⦄ := by
   exact coe_spec_EStateM_to_CompilerM (c_lookaround_PositiveLookbehind_spec _ _ _)
 
 @[spec] theorem c_lookaround_NegativeLookbehind_spec (next_char : Unchecked.StateID) (compiled : ThompsonRef) (states : Array Unchecked.State)
-    : ⦃fun s => ⌜s = states ∧ next_char < states.size ∧ tRefLt compiled states ∧ nextOfLt states⌝⦄
+    : ⦃fun s => ⌜s = states ∧ next_char < states.size ∧ tRefLt compiled states ∧ NextOfLt states⌝⦄
       Code.c_lookaround_NegativeLookbehind next_char compiled
       ⦃post⟨fun r s => ⌜tRefNextOfLeLt states r s⌝, fun _ => ⌜True⌝⟩⦄ := by
   mvcgen [Code.c_lookaround_NegativeLookbehind]
-  all_goals grind
+  with grind
 
 @[spec] theorem c_lookaround_NegativeLookbehind_lift_spec (next_char : Unchecked.StateID) (compiled : ThompsonRef) (states : Array Unchecked.State)
   (captures : Array NFA.Capture)
-    : ⦃fun s => ⌜(s.1 = states ∧ next_char < states.size ∧ tRefLt compiled states ∧ nextOfLt states)
+    : ⦃fun s => ⌜(s.1 = states ∧ next_char < states.size ∧ tRefLt compiled states ∧ NextOfLt states)
                 ∧ s.2.1 = captures ∧ cValid captures⌝⦄
       (Code.c_lookaround_NegativeLookbehind next_char compiled : Code.CompilerM ThompsonRef)
       ⦃post⟨fun r s => ⌜tRefNextOfLeLt states r s.1 ∧ s.2.1 = captures ∧ cMemAndValid captures s.2.1⌝, fun _ => ⌜True⌝⟩⦄ := by
   exact coe_spec_EStateM_to_CompilerM (c_lookaround_NegativeLookbehind_spec _ _ _)
 
 @[spec] theorem c_repetition_0_some_1_false_spec (union : Unchecked.StateID) (compiled : ThompsonRef) (states : Array Unchecked.State)
-    : ⦃fun s => ⌜s = states ∧ union < states.size ∧ tRefLt compiled states ∧ nextOfLt states⌝⦄
+    : ⦃fun s => ⌜s = states ∧ union < states.size ∧ tRefLt compiled states ∧ NextOfLt states⌝⦄
       Code.c_repetition_0_some_1_false union compiled
       ⦃post⟨fun r s => ⌜tRefNextOfLeLt states r s⌝, fun _ => ⌜True⌝⟩⦄ := by
   mvcgen [Code.c_repetition_0_some_1_false]
-  all_goals grind
+  with grind
 
 @[spec] theorem c_repetition_0_some_1_false_lift_spec (union : Unchecked.StateID) (compiled : ThompsonRef) (states : Array Unchecked.State)
   (captures : Array NFA.Capture)
-    : ⦃fun s => ⌜(s.1 = states ∧ union < states.size ∧ tRefLt compiled states ∧ nextOfLt states)
+    : ⦃fun s => ⌜(s.1 = states ∧ union < states.size ∧ tRefLt compiled states ∧ NextOfLt states)
                   ∧ s.2.1 = captures ∧ cValid captures⌝⦄
       (Code.c_repetition_0_some_1_false union compiled : Code.CompilerM ThompsonRef)
       ⦃post⟨fun r s => ⌜tRefNextOfLeLt states r s.1 ∧ s.2.1 = captures ∧ cMemAndValid captures s.2.1⌝, fun _ => ⌜True⌝⟩⦄ := by
   exact coe_spec_EStateM_to_CompilerM (c_repetition_0_some_1_false_spec _ _ _)
 
 @[spec] theorem c_repetition_0_some_1_true_spec (union : Unchecked.StateID) (compiled : ThompsonRef) (states : Array Unchecked.State)
-    : ⦃fun s => ⌜s = states ∧ union < states.size ∧ tRefLt compiled states ∧ nextOfLt states⌝⦄
+    : ⦃fun s => ⌜s = states ∧ union < states.size ∧ tRefLt compiled states ∧ NextOfLt states⌝⦄
       Code.c_repetition_0_some_1_true union compiled
       ⦃post⟨fun r s => ⌜tRefNextOfLeLt states r s⌝, fun _ => ⌜True⌝⟩⦄ := by
   mvcgen [Code.c_repetition_0_some_1_true]
-  all_goals simp_all [Unchecked.EatMode.nextOf] <;> grind
+  with grind
 
 @[spec] theorem c_repetition_0_some_1_true_lift_spec (union : Unchecked.StateID) (compiled : ThompsonRef) (states : Array Unchecked.State)
   (captures : Array NFA.Capture)
-    : ⦃fun s => ⌜(s.1 = states ∧ union < states.size ∧ tRefLt compiled states ∧ nextOfLt states)
+    : ⦃fun s => ⌜(s.1 = states ∧ union < states.size ∧ tRefLt compiled states ∧ NextOfLt states)
                 ∧ s.2.1 = captures ∧ cValid captures⌝⦄
       (Code.c_repetition_0_some_1_true union compiled : Code.CompilerM ThompsonRef)
       ⦃post⟨fun r s => ⌜tRefNextOfLeLt states r s.1 ∧ s.2.1 = captures ∧ cMemAndValid captures s.2.1⌝, fun _ => ⌜True⌝⟩⦄ := by
   exact coe_spec_EStateM_to_CompilerM (c_repetition_0_some_1_true_spec _ _ _)
 
 @[spec] theorem c_repetition_0_none_spec (union : Unchecked.StateID) (compiled : ThompsonRef) (states : Array Unchecked.State)
-    : ⦃fun s => ⌜s = states ∧ union < states.size ∧ tRefLt compiled states ∧ nextOfLt states⌝⦄
+    : ⦃fun s => ⌜s = states ∧ union < states.size ∧ tRefLt compiled states ∧ NextOfLt states⌝⦄
       Code.c_repetition_0_none union compiled
       ⦃post⟨fun r s => ⌜tRefNextOfLeLt states r s⌝, fun _ => ⌜True⌝⟩⦄ := by
   mvcgen [Code.c_repetition_0_none]
-  all_goals simp_all
+  with grind
 
 @[spec] theorem c_repetition_0_none_lift_spec (union : Unchecked.StateID) (compiled : ThompsonRef) (states : Array Unchecked.State)
   (captures : Array NFA.Capture)
-    : ⦃fun s => ⌜(s.1 = states ∧ union < states.size ∧ tRefLt compiled states ∧ nextOfLt states)
+    : ⦃fun s => ⌜(s.1 = states ∧ union < states.size ∧ tRefLt compiled states ∧ NextOfLt states)
                   ∧ s.2.1 = captures ∧ cValid captures⌝⦄
       (Code.c_repetition_0_none union compiled : Code.CompilerM ThompsonRef)
       ⦃post⟨fun r s => ⌜tRefNextOfLeLt states r s.1 ∧ s.2.1 = captures ∧ cMemAndValid captures s.2.1⌝, fun _ => ⌜True⌝⟩⦄ := by
   exact coe_spec_EStateM_to_CompilerM (c_repetition_0_none_spec _ _ _)
 
 @[spec] theorem greedy_union_spec (greedy : Bool) (states : Array Unchecked.State)
-    : ⦃fun s => ⌜s = states ∧ nextOfLt states⌝⦄
+    : ⦃fun s => ⌜s = states ∧ NextOfLt states⌝⦄
       (if greedy then Code.add_union else Code.add_union_reverse : Code.PatchM Unchecked.StateID)
       ⦃post⟨fun r s => ⌜stateIdNextOfLt states r s⌝, fun _ => ⌜True⌝⟩⦄ := by
   split <;> mvcgen
 
 @[spec] theorem c_at_least_0_pre_spec (compiled : ThompsonRef) (greedy : Bool) (states : Array Unchecked.State)
-    : ⦃fun s => ⌜s = states ∧ tRefLt compiled states ∧ nextOfLt states⌝⦄
+    : ⦃fun s => ⌜s = states ∧ tRefLt compiled states ∧ NextOfLt states⌝⦄
       Code.c_at_least_0_pre compiled greedy
       ⦃post⟨fun r s => ⌜stateIdNextOfLt states r s⌝, fun _ => ⌜True⌝⟩⦄ := by
   mvcgen [Code.c_at_least_0_pre]
-  all_goals simp_all <;> grind
+  with grind
 
 @[spec] theorem c_at_least_0_pre_lift_spec (compiled : ThompsonRef) (greedy : Bool) (states : Array Unchecked.State)
   (captures : Array NFA.Capture)
-    : ⦃fun s => ⌜(s.1 = states ∧ tRefLt compiled states ∧ nextOfLt states)
+    : ⦃fun s => ⌜(s.1 = states ∧ tRefLt compiled states ∧ NextOfLt states)
                 ∧ s.2.1 = captures ∧ cValid captures⌝⦄
       (Code.c_at_least_0_pre compiled greedy : Code.CompilerM Unchecked.StateID)
       ⦃post⟨fun r s => ⌜stateIdNextOfLt states r s.1 ∧ s.2.1 = captures ∧ cMemAndValid captures s.2.1⌝, fun _ => ⌜True⌝⟩⦄ := by
@@ -697,19 +709,27 @@ theorem c_possessive_le_lift_spec (tref : ThompsonRef) (states : Array Unchecked
       Code.c_at_least_set possible_empty_capture_group greedy
       ⦃post⟨fun _ s => ⌜states = s.1  ∧ groups.size ≤ s.2.2.size⌝, fun _ => ⌜True⌝⟩⦄ := by
   mvcgen [Code.c_at_least_set]
-  split <;> simp_all
+  with grind
 
 @[spec] theorem c_at_least_0_post_spec (compiled : ThompsonRef) (plus : Unchecked.StateID) (greedy : Bool)
   (possessive : Bool) (states : Array Unchecked.State)
-    : ⦃fun s => ⌜s = states ∧ plus < states.size ∧ compiled.start < states.size ∧ nextOfLt states⌝⦄
+    : ⦃fun s => ⌜s = states ∧ plus < states.size ∧ compiled.start < states.size ∧ NextOfLt states⌝⦄
       Code.c_at_least_0_post compiled plus greedy possessive
       ⦃post⟨fun r s => ⌜tRefNextOfLeLt states r s⌝, fun _ => ⌜True⌝⟩⦄ := by
   mvcgen [Code.c_at_least_0_post]
-  all_goals inst_mvar <;> grind
+  case vc11 =>
+    and_intros
+    rfl
+    all_goals grind
+  case vc25 =>
+    and_intros
+    rfl
+    all_goals grind
+  all_goals grind
 
 @[spec] theorem c_at_least_0_post_lift_spec (compiled : ThompsonRef) (plus : Unchecked.StateID) (greedy : Bool)
   (possessive : Bool) (states : Array Unchecked.State) (captures : Array NFA.Capture)
-    : ⦃fun s => ⌜(s.1 = states ∧ plus < states.size ∧ compiled.start < states.size ∧ nextOfLt states)
+    : ⦃fun s => ⌜(s.1 = states ∧ plus < states.size ∧ compiled.start < states.size ∧ NextOfLt states)
                 ∧ s.2.1 = captures ∧ cValid captures⌝⦄
       (Code.c_at_least_0_post compiled plus greedy possessive : Code.CompilerM ThompsonRef)
       ⦃post⟨fun r s => ⌜tRefNextOfLeLt states r s.1 ∧ s.2.1 = captures ∧ cMemAndValid captures s.2.1⌝, fun _ => ⌜True⌝⟩⦄ := by
@@ -717,36 +737,43 @@ theorem c_possessive_le_lift_spec (tref : ThompsonRef) (states : Array Unchecked
 
 @[spec] theorem c_at_least_0_spec (compiled : ThompsonRef) (possible_empty_capture_group : Option Nat) (greedy : Bool)
   (states : Array Unchecked.State) (captures : Array NFA.Capture)
-    : ⦃fun s => ⌜s.1 = states ∧ tRefLt compiled states ∧ nextOfLt states ∧ s.2.1 = captures ∧ cValid captures⌝⦄
+    : ⦃fun s => ⌜s.1 = states ∧ tRefLt compiled states ∧ NextOfLt states ∧ s.2.1 = captures ∧ cValid captures⌝⦄
       Code.c_at_least_0 compiled possible_empty_capture_group greedy
       ⦃post⟨fun r s => ⌜stateIdNextOfLt states r s.1 ∧ s.2.1 = captures ∧ cMemAndValid captures s.2.1⌝, fun _ => ⌜True⌝⟩⦄ := by
   mvcgen [Code.c_at_least_0]
-  grind
+  with grind
 
 @[spec] theorem c_at_least_1_pre_spec (greedy : Bool) (states : Array Unchecked.State)
-    : ⦃fun s => ⌜s = states ∧ nextOfLt states⌝⦄
+    : ⦃fun s => ⌜s = states ∧ NextOfLt states⌝⦄
       Code.c_at_least_1_pre greedy
       ⦃post⟨fun r s => ⌜stateIdNextOfLt states r s⌝, fun _ => ⌜True⌝⟩⦄ := by
   mvcgen [Code.c_at_least_1_pre]
 
 @[spec] theorem c_at_least_1_pre_lift_spec (greedy : Bool) (states : Array Unchecked.State)
   (captures : Array NFA.Capture)
-    : ⦃fun s => ⌜(s.1 = states ∧ nextOfLt states) ∧ s.2.1 = captures ∧ cValid captures⌝⦄
+    : ⦃fun s => ⌜(s.1 = states ∧ NextOfLt states) ∧ s.2.1 = captures ∧ cValid captures⌝⦄
       (Code.c_at_least_1_pre greedy : Code.CompilerM Unchecked.StateID)
       ⦃post⟨fun r s => ⌜stateIdNextOfLt states r s.1 ∧ s.2.1 = captures ∧ cMemAndValid captures s.2.1⌝, fun _ => ⌜True⌝⟩⦄ := by
   exact coe_spec_EStateM_to_CompilerM (c_at_least_1_pre_spec _ _)
 
 @[spec] theorem c_at_least_1_post_spec (compiled : ThompsonRef) (union : Unchecked.StateID)
   (possessive : Bool) (states : Array Unchecked.State)
-    : ⦃fun s => ⌜s = states ∧ union < states.size ∧ tRefLt compiled states ∧ nextOfLt states⌝⦄
+    : ⦃fun s => ⌜s = states ∧ union < states.size ∧ tRefLt compiled states ∧ NextOfLt states⌝⦄
       Code.c_at_least_1_post compiled union possessive
       ⦃post⟨fun r s => ⌜tRefNextOfLeLt states r s⌝, fun _ => ⌜True⌝⟩⦄ := by
   mvcgen [Code.c_at_least_1_post]
-  all_goals (inst_mvar <;> try simp_all) <;> grind
+  case vc5.post.success =>
+    and_intros
+    rfl
+    grind
+    grind
+    apply NextOfLt.mk
+    grind
+  all_goals grind
 
 @[spec] theorem c_at_least_1_post_lift_spec (compiled : ThompsonRef) (union : Unchecked.StateID)
   (possessive : Bool) (states : Array Unchecked.State) (captures : Array NFA.Capture)
-    : ⦃fun s => ⌜(s.1 = states ∧ union < states.size ∧ tRefLt compiled states ∧ nextOfLt states)
+    : ⦃fun s => ⌜(s.1 = states ∧ union < states.size ∧ tRefLt compiled states ∧ NextOfLt states)
                   ∧ s.2.1 = captures ∧ cValid captures⌝⦄
       (Code.c_at_least_1_post compiled union possessive : Code.CompilerM ThompsonRef)
       ⦃post⟨fun r s => ⌜tRefNextOfLeLt states r s.1 ∧ s.2.1 = captures ∧ cMemAndValid captures s.2.1⌝, fun _ => ⌜True⌝⟩⦄ := by
@@ -754,22 +781,30 @@ theorem c_possessive_le_lift_spec (tref : ThompsonRef) (states : Array Unchecked
 
 @[spec] theorem c_at_least_1_spec (possible_empty_capture_group : Option Nat) (greedy : Bool)
   (states : Array Unchecked.State) (captures : Array NFA.Capture)
-    : ⦃fun s => ⌜(s.1 = states ∧ nextOfLt states) ∧ s.2.1 = captures ∧ cValid captures⌝⦄
+    : ⦃fun s => ⌜(s.1 = states ∧ NextOfLt states) ∧ s.2.1 = captures ∧ cValid captures⌝⦄
       Code.c_at_least_1 possible_empty_capture_group greedy
       ⦃post⟨fun r s => ⌜stateIdNextOfLt states r s.1 ∧ s.2.1 = captures ∧ cMemAndValid captures s.2.1⌝, fun _ => ⌜True⌝⟩⦄ := by
   mvcgen [Code.c_at_least_1]
 
 @[spec] theorem c_at_least_2_spec («prefix» last : ThompsonRef) (greedy : Bool)
   (possessive : Bool) (states : Array Unchecked.State)
-    : ⦃fun s => ⌜s = states ∧ tRefLt «prefix» states ∧ tRefLt last states ∧ nextOfLt states⌝⦄
+    : ⦃fun s => ⌜s = states ∧ tRefLt «prefix» states ∧ tRefLt last states ∧ NextOfLt states⌝⦄
       Code.c_at_least_2 «prefix» last greedy possessive
       ⦃post⟨fun r s => ⌜tRefNextOfLeLt states r s⌝, fun _ => ⌜True⌝⟩⦄ := by
   mvcgen [Code.c_at_least_2]
-  all_goals inst_mvar <;> grind
+  case vc9 =>
+    and_intros
+    rfl
+    all_goals grind
+  case vc21 =>
+    and_intros
+    rfl
+    all_goals grind
+  all_goals grind
 
 @[spec] theorem c_at_least_2_lift_spec («prefix» last : ThompsonRef) (greedy : Bool)
   (possessive : Bool) (states : Array Unchecked.State) (captures : Array NFA.Capture)
-    : ⦃fun s => ⌜(s.1 = states ∧ tRefLt «prefix» states ∧ tRefLt last states ∧ nextOfLt states)
+    : ⦃fun s => ⌜(s.1 = states ∧ tRefLt «prefix» states ∧ tRefLt last states ∧ NextOfLt states)
                   ∧ s.2.1 = captures ∧ cValid captures⌝⦄
       (Code.c_at_least_2 «prefix» last greedy possessive : Code.CompilerM ThompsonRef)
       ⦃post⟨fun r s => ⌜tRefNextOfLeLt states r s.1 ∧ s.2.1 = captures ∧ cMemAndValid captures s.2.1⌝, fun _ => ⌜True⌝⟩⦄ := by
@@ -778,42 +813,49 @@ theorem c_possessive_le_lift_spec (tref : ThompsonRef) (states : Array Unchecked
 @[spec] theorem c_bounded.fold.patch.pre_spec (compiled: ThompsonRef) (prev_end : Unchecked.StateID)
   (greedy : Bool) (states : Array Unchecked.State)
     : ⦃fun s => ⌜s = states ∧ tRefLt compiled states
-                      ∧ prev_end < states.size ∧ nextOfLt states⌝⦄
+                      ∧ prev_end < states.size ∧ NextOfLt states⌝⦄
       Code.c_bounded.fold.patch.pre compiled prev_end greedy
       ⦃post⟨fun r s => ⌜stateIdNextOfLt states r s⌝, fun _ => ⌜True⌝⟩⦄ := by
   mvcgen [Code.c_bounded.fold.patch.pre]
-  all_goals simp_all <;> grind
+  all_goals grind
 
 @[spec] theorem c_bounded.fold.patch.possessive_spec (compiled: ThompsonRef) (empty : Unchecked.StateID)
   (states : Array Unchecked.State)
     : ⦃fun s => ⌜s = states ∧ tRefLt compiled states
-                      ∧ empty < states.size ∧ nextOfLt states⌝⦄
+                      ∧ empty < states.size ∧ NextOfLt states⌝⦄
       Code.c_bounded.fold.patch.possessive compiled empty
       ⦃post⟨fun r s => ⌜stateIdNextOfLeLt states r s⌝, fun _ => ⌜True⌝⟩⦄ := by
   mvcgen [Code.c_bounded.fold.patch.possessive]
-  all_goals inst_mvar <;> grind
+  with grind
 
 @[spec] theorem c_bounded.fold.patch.post_spec (compiled: ThompsonRef) (union empty : Unchecked.StateID) (states : Array Unchecked.State)
     : ⦃fun s => ⌜s = states ∧ compiled.end < states.size
-                      ∧ union < states.size ∧ empty < states.size ∧ nextOfLt states⌝⦄
+                      ∧ union < states.size ∧ empty < states.size ∧ NextOfLt states⌝⦄
       Code.c_bounded.fold.patch.post compiled union empty
       ⦃post⟨fun r s => ⌜stateIdNextOfLeLt states r s⌝, fun _ => ⌜True⌝⟩⦄ := by
   mvcgen [Code.c_bounded.fold.patch.post]
-  all_goals grind
+  with grind
 
 @[spec] theorem c_bounded.fold.patch_spec (compiled: ThompsonRef) (prev_end empty : Unchecked.StateID)
   (greedy : Bool) (possessive : Bool) (states : Array Unchecked.State)
     : ⦃fun s => ⌜s = states ∧ tRefLt compiled states
-                      ∧ prev_end < states.size ∧ empty < states.size ∧ nextOfLt states⌝⦄
+                      ∧ prev_end < states.size ∧ empty < states.size ∧ NextOfLt states⌝⦄
       Code.c_bounded.fold.patch compiled prev_end empty greedy possessive
       ⦃post⟨fun r s => ⌜stateIdNextOfLt states r s⌝, fun _ => ⌜True⌝⟩⦄ := by
   mvcgen [Code.c_bounded.fold.patch]
-  all_goals inst_mvar <;> grind
+  case vc3 =>
+    inst_mvar
+    all_goals grind
+  case vc6 =>
+    and_intros
+    rfl
+    all_goals grind
+  all_goals grind
 
 @[spec] theorem c_bounded.fold.patch_lift_spec  (compiled: ThompsonRef) (prev_end empty : Unchecked.StateID)
   (greedy : Bool) (possessive : Bool) (states : Array Unchecked.State) (captures : Array NFA.Capture)
     : ⦃fun s => ⌜(s.1 = states ∧ tRefLt compiled states
-                      ∧ prev_end < states.size ∧ empty < states.size ∧ nextOfLt states)
+                      ∧ prev_end < states.size ∧ empty < states.size ∧ NextOfLt states)
                   ∧ s.2.1 = captures ∧ cValid captures⌝⦄
       (Code.c_bounded.fold.patch compiled prev_end empty greedy possessive : Code.CompilerM Unchecked.StateID)
       ⦃post⟨fun r s => ⌜stateIdNextOfLt states r s.1 ∧ s.2.1 = captures ∧ cMemAndValid captures s.2.1⌝, fun _ => ⌜True⌝⟩⦄ := by
@@ -821,29 +863,29 @@ theorem c_possessive_le_lift_spec (tref : ThompsonRef) (states : Array Unchecked
 
 @[spec] theorem c_alt_iter_step_spec (first second: ThompsonRef) (states : Array Unchecked.State)
     : ⦃fun s => ⌜s = states ∧ tRefLt first states
-                      ∧ tRefLt second states ∧ nextOfLt states⌝⦄
+                      ∧ tRefLt second states ∧ NextOfLt states⌝⦄
       Code.c_alt_iter_step first second
       ⦃post⟨fun r s => ⌜tRefNextOfLt states ⟨r.1, r.2⟩ s⌝, fun _ => ⌜True⌝⟩⦄ := by
   mvcgen [Code.c_alt_iter_step]
-  all_goals grind
+  with grind
 
 @[spec] theorem c_alt_iter_step_lift_spec (first second: ThompsonRef) (states : Array Unchecked.State)
   (captures : Array NFA.Capture)
-    : ⦃fun s => ⌜(s.1 = states ∧ tRefLt first states ∧ tRefLt second states ∧ nextOfLt states)
+    : ⦃fun s => ⌜(s.1 = states ∧ tRefLt first states ∧ tRefLt second states ∧ NextOfLt states)
                 ∧ s.2.1 = captures ∧ cValid captures⌝⦄
       (Code.c_alt_iter_step first second : Code.CompilerM (Unchecked.StateID × Unchecked.StateID))
       ⦃post⟨fun r s => ⌜tRefNextOfLt states ⟨r.1, r.2⟩ s.1 ∧ s.2.1 = captures ∧ cMemAndValid captures s.2.1⌝, fun _ => ⌜True⌝⟩⦄ := by
   exact coe_spec_EStateM_to_CompilerM (c_alt_iter_step_spec _ _ _)
 
 @[spec] theorem c_rep_pre_spec (greedy : Bool) (states : Array Unchecked.State)
-    : ⦃fun s => ⌜s = states ∧ nextOfLt states⌝⦄
+    : ⦃fun s => ⌜s = states ∧ NextOfLt states⌝⦄
       Code.c_rep_pre greedy
       ⦃post⟨fun r s => ⌜stateIdNextOfLt states r s⌝, fun _ => ⌜True⌝⟩⦄ := by
   mvcgen [Code.c_rep_pre]
 
 @[spec] theorem c_rep_pre_lift_spec (greedy : Bool) (states : Array Unchecked.State)
   (captures : Array NFA.Capture)
-    : ⦃fun s => ⌜(s.1 = states ∧ nextOfLt states) ∧ s.2.1 = captures ∧ cValid captures⌝⦄
+    : ⦃fun s => ⌜(s.1 = states ∧ NextOfLt states) ∧ s.2.1 = captures ∧ cValid captures⌝⦄
       (Code.c_rep_pre greedy : Code.CompilerM Unchecked.StateID)
       ⦃post⟨fun r s => ⌜stateIdNextOfLt states r s.1 ∧ s.2.1 = captures ∧ cMemAndValid captures s.2.1⌝, fun _ => ⌜True⌝⟩⦄ := by
   exact coe_spec_EStateM_to_CompilerM (c_rep_pre_spec _ _)
@@ -852,16 +894,146 @@ set_option maxHeartbeats 4000000
 
 mutual
 
+@[spec] theorem c_bounded_spec (hir : Hir) (min max : Nat) (greedy : Bool) (possessive : Bool)
+  (states : Array Unchecked.State) (captures : Array NFA.Capture)
+    : ⦃fun s => ⌜s.1 = states ∧  NextOfLt states ∧ s.2.1 = captures ∧ cValid captures⌝⦄
+      Code.c_bounded hir min max greedy possessive
+      ⦃post⟨fun r s => ⌜tRefNextOfLt states r s.1 ∧ cMemAndValid captures s.2.1⌝, fun _ => ⌜True⌝⟩⦄ := by
+  mintro _
+  unfold Code.c_bounded
+  split
+  mspec c_exactly_spec
+  split
+  case isTrue.post.success.isTrue =>
+    split
+    · mspec c_possessive_le_lift_spec
+      inst_mvars
+      case post.success => mvcgen with grind
+      all_goals grind
+    · simp_all
+  case isTrue.post.success.isFalse =>
+      mspec add_empty_lift'_spec
+      inst_mvars
+      case post.success =>
+        mspec c_bounded_fold_spec
+        inst_mvars
+        case post.success =>
+          mspec patch_lift_spec
+          · inst_mvars
+            all_goals grind
+          · mvcgen with grind [= cValid, = cMemAndValid]
+        all_goals grind
+      all_goals grind
+  case isFalse =>
+    mspec c_empty_lift_spec
+    inst_mvars
+    case post.success => mvcgen with grind
+    all_goals grind
+termination_by sizeOf hir + sizeOf min + sizeOf (max - min) + 1
+
+@[spec] theorem c_lookaround_spec (look : Lookaround) (states : Array Unchecked.State)
+  (captures : Array NFA.Capture)
+    : ⦃fun s => ⌜s.1 = states ∧ NextOfLt states ∧ s.2.1 = captures ∧ cValid captures⌝⦄
+      Code.c_lookaround look
+      ⦃post⟨fun r s => ⌜tRefNextOfLt states r s.1 ∧ cMemAndValid captures s.2.1⌝, fun _ => ⌜True⌝⟩⦄ := by
+  mintro _
+  unfold Code.c_lookaround
+  split
+  case h_1 | h_2 =>
+    mspec c_spec
+    mspec
+    inst_mvars
+    all_goals simp_all
+    all_goals grind
+  case h_3 | h_4 =>
+    mspec add_next_char_lift_spec
+    inst_mvars
+    case post.success =>
+      mspec c_spec
+      inst_mvars
+      case post.success =>
+        mspec
+        inst_mvars
+        case post.success => simp; intros; grind
+        all_goals simp_all
+        all_goals grind
+      all_goals grind
+    all_goals grind
+termination_by sizeOf look
+
+@[spec] theorem c_repetition_spec (rep : Repetition) (states : Array Unchecked.State)
+  (captures : Array NFA.Capture)
+    : ⦃fun s => ⌜s.1 = states ∧ NextOfLt states ∧ s.2.1 = captures ∧ cValid captures⌝⦄
+      Code.c_repetition rep
+      ⦃post⟨fun r s => ⌜tRefNextOfLt states r s.1 ∧ cMemAndValid captures s.2.1⌝, fun _ => ⌜True⌝⟩⦄ := by
+  mintro _
+  unfold Code.c_repetition
+  split
+  case h_1 | h_2 =>
+    mspec
+    inst_mvars
+    case post.success =>
+      mspec c_spec
+      inst_mvars
+      case post.success =>
+        mspec
+        inst_mvars
+        case post.success => mvcgen with grind
+        all_goals grind
+      all_goals grind
+    all_goals grind
+  case h_3 =>
+    split
+    · mspec
+      inst_mvars
+      case post.success =>
+        mspec c_spec
+        inst_mvars
+        case post.success =>
+          mspec
+          inst_mvars
+          case post.success => mvcgen with grind
+          all_goals grind
+        all_goals grind
+      all_goals grind
+    · mspec c_at_least_spec
+  case h_4 =>
+    split
+    mspec c_bounded_spec
+    inst_mvars
+    intros
+    mvcgen with grind
+termination_by sizeOf rep
+
+@[spec] theorem c_exactly_spec (hir : Hir) (n : Nat) (states : Array Unchecked.State)
+   (captures : Array NFA.Capture)
+    : ⦃fun s => ⌜s.1 = states ∧  NextOfLt states ∧ s.2.1 = captures ∧ cValid captures⌝⦄
+      Code.c_exactly hir n
+      ⦃post⟨fun r s => ⌜tRefNextOfLt states r s.1 ∧ cMemAndValid captures s.2.1⌝, fun _ => ⌜True⌝⟩⦄ := by
+  mintro _
+  unfold Code.c_exactly
+  split
+  · mspec c_spec
+    mspec c_exactly_fold_spec
+    inst_mvars
+    case isTrue.post.success.post.success => mvcgen with grind [= cValid, = cMemAndValid]
+    all_goals grind
+  · mspec c_empty_lift_spec
+    inst_mvars
+    case isFalse.post.success => mvcgen with grind
+    all_goals grind
+termination_by sizeOf hir + sizeOf n
+
 @[spec] theorem c_concat_fold_spec (tail : Array Hir) (sid : Unchecked.StateID)
  (states : Array Unchecked.State) (captures : Array NFA.Capture)
-    : ⦃fun s => ⌜(s.1 = states ∧ sid < states.size ∧ nextOfLt states) ∧ s.2.1 = captures ∧ cValid captures⌝⦄
+    : ⦃fun s => ⌜(s.1 = states ∧ sid < states.size ∧ NextOfLt states) ∧ s.2.1 = captures ∧ cValid captures⌝⦄
       Code.c_concat.fold tail sid
       ⦃post⟨fun r s => ⌜stateIdNextOfLeLt states r s.1 ∧ cMemAndValid captures s.2.1⌝, fun _ => ⌜True⌝⟩⦄ := by
   mintro _
   unfold Code.c_concat.fold
   mspec Spec.foldlM_array
   case inv =>
-    exact (fun (xs, r) s => ⌜states.size ≤ s.1.size ∧ sid < s.1.size ∧ r < s.1.size ∧ nextOfLt s.1
+    exact (fun (xs, r) s => ⌜states.size ≤ s.1.size ∧ sid < s.1.size ∧ r < s.1.size ∧ NextOfLt s.1
                               ∧ cMemAndValid captures s.2.1⌝, fun e => ⌜true⌝, ())
   case step =>
     intros
@@ -873,19 +1045,16 @@ mutual
     case post.success =>
       mspec patch_lift_spec
       · inst_mvars
-        simp_all; grind; grind; all_goals simp_all
-      · simp
-        grind
-    all_goals simp_all
-  case pre =>
-    simp
-    intros
-    and_intros <;> simp_all
-  all_goals simp_all
+        all_goals grind
+      · mvcgen
+        grind [= cMemAndValid]
+    all_goals grind
+  case pre => simp_all
+  simp_all
 termination_by sizeOf tail
 
 @[spec] theorem c_concat_spec (hirs : Array Hir) (states : Array Unchecked.State) (captures : Array NFA.Capture)
-    : ⦃fun s => ⌜(s.1 = states ∧ nextOfLt states) ∧ s.2.1 = captures ∧ cValid captures⌝⦄
+    : ⦃fun s => ⌜(s.1 = states ∧ NextOfLt states) ∧ s.2.1 = captures ∧ cValid captures⌝⦄
       Code.c_concat hirs
       ⦃post⟨fun r s => ⌜tRefNextOfLt states r s.1 ∧ cMemAndValid captures s.2.1⌝, fun _ => ⌜True⌝⟩⦄ := by
   mintro _
@@ -899,18 +1068,17 @@ termination_by sizeOf tail
   case h_1.post.success =>
     mspec c_concat_fold_spec
     inst_mvars
-    grind; simp_all; simp_all; simp_all; simp_all; simp_all; grind
-  all_goals simp_all
-  intros
-  mvcgen
-  · and_intros
-    all_goals simp_all
-  · simp_all
+    case post.success =>
+      mvcgen with grind [= cValid, = cMemAndValid]
+    all_goals grind
+  case h_2 =>
+    mvcgen with grind
+  all_goals grind
 termination_by sizeOf hirs
 
 @[spec] theorem c_alt_iter_fold_spec (hirs : Array Hir) (union «end» : Unchecked.StateID)
   (states : Array Unchecked.State) (captures : Array NFA.Capture)
-    : ⦃fun s => ⌜s.1 = states ∧ union < states.size ∧ «end» < states.size ∧ nextOfLt states
+    : ⦃fun s => ⌜s.1 = states ∧ union < states.size ∧ «end» < states.size ∧ NextOfLt states
                 ∧ s.2.1 = captures ∧ cValid captures⌝⦄
       Code.c_alt_iter.fold hirs union «end»
       ⦃post⟨fun _ s => ⌜statesNextOfLeLt states s.1  ∧ cMemAndValid captures s.2.1⌝, fun _ => ⌜True⌝⟩⦄ := by
@@ -919,7 +1087,7 @@ termination_by sizeOf hirs
   mspec Spec.foldlM_array
   case inv =>
     exact (fun (_, xs) s => ⌜states.size ≤ s.1.size ∧ union < s.1.size ∧ «end» < s.1.size
-                              ∧ nextOfLt s.1 ∧ cMemAndValid captures s.2.1⌝, fun e => ⌜true⌝, ())
+                              ∧ NextOfLt s.1 ∧ cMemAndValid captures s.2.1⌝, fun e => ⌜true⌝, ())
   case step =>
     intros
     expose_names
@@ -933,10 +1101,11 @@ termination_by sizeOf hirs
       case post.success =>
         mspec patch_lift_spec
         inst_mvars
-        case post.success => simp; intros; grind
-        simp_all; grind; grind; all_goals simp_all
-      simp_all; grind; grind; all_goals simp_all
-    all_goals simp_all
+        case post.success =>
+          mvcgen with grind [= cMemAndValid]
+        all_goals grind
+      all_goals grind
+    all_goals grind
   case pre =>
     simp_all
   case post =>
@@ -945,7 +1114,7 @@ termination_by sizeOf hirs
 
 @[spec] theorem c_alt_iter_spec (hirs : Array Hir) (states : Array Unchecked.State)
   (captures : Array NFA.Capture)
-    : ⦃fun s => ⌜s.1 = states ∧  nextOfLt states ∧ s.2.1 = captures ∧ cValid captures⌝⦄
+    : ⦃fun s => ⌜s.1 = states ∧  NextOfLt states ∧ s.2.1 = captures ∧ cValid captures⌝⦄
       Code.c_alt_iter hirs
       ⦃post⟨fun r s => ⌜tRefNextOfLt states r s.1 ∧ cMemAndValid captures s.2.1⌝, fun _ => ⌜True⌝⟩⦄ := by
   mintro _
@@ -969,10 +1138,10 @@ termination_by sizeOf hirs
         case post.success =>
           mspec c_alt_iter_fold_spec
           inst_mvars
-          case post.success => simp; intros; grind
-          grind; grind; all_goals simp_all
-        grind; grind; all_goals simp_all
-      all_goals simp_all
+          case post.success => mvcgen with grind [= cMemAndValid]
+          all_goals grind
+        all_goals grind
+      all_goals grind
     case h_2 =>
       simp_all [wp]
   case h_2 =>
@@ -981,7 +1150,7 @@ termination_by sizeOf hirs
 
 @[spec] theorem c_exactly_fold_spec (hir : Hir) (n : Nat) («end» : Unchecked.StateID)
   (states : Array Unchecked.State) (captures : Array NFA.Capture)
-    : ⦃fun s => ⌜s.1 = states ∧ «end» < states.size ∧  nextOfLt states
+    : ⦃fun s => ⌜s.1 = states ∧ «end» < states.size ∧  NextOfLt states
                   ∧ s.2.1 = captures ∧ cValid captures⌝⦄
       Code.c_exactly.fold hir n «end»
       ⦃post⟨fun r s => ⌜stateIdNextOfLeLt states r s.1 ∧ cMemAndValid captures s.2.1⌝, fun _ => ⌜True⌝⟩⦄ := by
@@ -991,7 +1160,7 @@ termination_by sizeOf hirs
   mspec Spec.foldlM_list
   case inv =>
     exact (fun (xs, r) s => ⌜states.size ≤ s.1.size ∧ r < s.1.size ∧ «end» < s.1.size
-                              ∧ nextOfLt s.1 ∧ cMemAndValid captures s.2.1⌝, fun e => ⌜true⌝, ())
+                              ∧ NextOfLt s.1 ∧ cMemAndValid captures s.2.1⌝, fun e => ⌜true⌝, ())
   case step =>
     intros
     mintro _
@@ -1000,33 +1169,15 @@ termination_by sizeOf hirs
     case post.success =>
       mspec patch_lift_spec
       inst_mvars
-      case post.success => inst_mvars; grind
-      simp_all; grind; all_goals simp_all
-    all_goals simp_all
+      case post.success => mvcgen with grind [= cMemAndValid]
+      all_goals grind
+    all_goals grind
   all_goals simp_all
-termination_by sizeOf hir + sizeOf n
-
-@[spec] theorem c_exactly_spec (hir : Hir) (n : Nat) (states : Array Unchecked.State)
-   (captures : Array NFA.Capture)
-    : ⦃fun s => ⌜s.1 = states ∧  nextOfLt states ∧ s.2.1 = captures ∧ cValid captures⌝⦄
-      Code.c_exactly hir n
-      ⦃post⟨fun r s => ⌜tRefNextOfLt states r s.1 ∧ cMemAndValid captures s.2.1⌝, fun _ => ⌜True⌝⟩⦄ := by
-  mintro _
-  unfold Code.c_exactly
-  split
-  · mspec c_spec
-    mspec c_exactly_fold_spec
-    inst_mvars
-    case isTrue.post.success.post.success => inst_mvars; grind
-    grind; all_goals simp_all
-  · mspec c_empty_lift_spec
-    inst_mvars
-    all_goals simp_all
 termination_by sizeOf hir + sizeOf n
 
 @[spec] theorem c_at_least_spec (hir : Hir) (n : Nat) (greedy : Bool) (possessive : Bool)
   (states : Array Unchecked.State) (captures : Array NFA.Capture)
-    : ⦃fun s => ⌜s.1 = states ∧  nextOfLt states ∧ s.2.1 = captures ∧ cValid captures⌝⦄
+    : ⦃fun s => ⌜s.1 = states ∧  NextOfLt states ∧ s.2.1 = captures ∧ cValid captures⌝⦄
       Code.c_at_least hir n greedy possessive
       ⦃post⟨fun r s => ⌜tRefNextOfLt states r s.1 ∧ cMemAndValid captures s.2.1⌝, fun _ => ⌜True⌝⟩⦄ := by
   mintro _
@@ -1039,9 +1190,9 @@ termination_by sizeOf hir + sizeOf n
     case post.success.post.success =>
       mspec c_at_least_0_post_lift_spec
       inst_mvars
-      case post.success => simp; intros; grind
-      grind; grind; all_goals simp_all
-    all_goals simp_all
+      case post.success => mvcgen with grind
+      all_goals grind
+    all_goals grind
   case isFalse =>
     split
     mspec c_spec
@@ -1051,7 +1202,7 @@ termination_by sizeOf hir + sizeOf n
       mspec c_at_least_1_post_lift_spec
       inst_mvars
       case post.success => simp; intros; grind
-      grind; grind; grind; all_goals simp_all
+      all_goals grind
     case isFalse =>
       mspec c_exactly_spec
       mspec c_spec
@@ -1059,15 +1210,15 @@ termination_by sizeOf hir + sizeOf n
       case post.success.post.success =>
         mspec c_at_least_2_lift_spec
         inst_mvars
-        case post.success => simp; intros; grind
-        grind; grind; grind; grind; all_goals simp_all
-      all_goals simp_all
-    all_goals simp_all
+        case post.success => simp; intros; grind [= cMemAndValid]
+        all_goals grind
+      all_goals grind
+    all_goals grind
 termination_by sizeOf hir + sizeOf n + 1
 
 @[spec] theorem c_bounded_fold_spec  (hir : Hir) (n : Nat) («prefix» : ThompsonRef) (empty : Unchecked.StateID)
   (greedy : Bool) (possessive : Bool) (states : Array Unchecked.State) (captures : Array NFA.Capture)
-    : ⦃fun s => ⌜s.1 = states ∧ tRefLt «prefix» states ∧ empty < states.size ∧ nextOfLt states
+    : ⦃fun s => ⌜s.1 = states ∧ tRefLt «prefix» states ∧ empty < states.size ∧ NextOfLt states
                  ∧ s.2.1 = captures ∧ cValid captures⌝⦄
       Code.c_bounded.fold hir n «prefix» empty greedy possessive
       ⦃post⟨fun r s => ⌜stateIdNextOfLeLt states r s.1 ∧ cMemAndValid captures s.2.1⌝, fun _ => ⌜True⌝⟩⦄ := by
@@ -1077,7 +1228,7 @@ termination_by sizeOf hir + sizeOf n + 1
   mspec Spec.foldlM_list
   case inv =>
     exact (fun (xs, r) s => ⌜states.size ≤ s.1.size ∧ r < s.1.size ∧ empty < s.1.size
-                            ∧ nextOfLt s.1 ∧ cMemAndValid captures s.2.1⌝, fun e => ⌜true⌝, ())
+                            ∧ NextOfLt s.1 ∧ cMemAndValid captures s.2.1⌝, fun e => ⌜true⌝, ())
   case step =>
     intros
     mintro _
@@ -1086,9 +1237,9 @@ termination_by sizeOf hir + sizeOf n + 1
     case post.success =>
       mspec c_bounded.fold.patch_lift_spec
       inst_mvars
-      case post.success => simp; intros; grind
-      grind; grind; grind; grind; all_goals simp_all
-    all_goals simp_all
+      case post.success => mvcgen with grind [= cMemAndValid]
+      all_goals grind
+    all_goals grind
   case pre =>
     intro _
     simp_all
@@ -1100,119 +1251,9 @@ termination_by sizeOf hir + sizeOf n + 1
     simp_all
 termination_by sizeOf hir + sizeOf n
 
-@[spec] theorem c_bounded_spec (hir : Hir) (min max : Nat) (greedy : Bool) (possessive : Bool)
-  (states : Array Unchecked.State) (captures : Array NFA.Capture)
-    : ⦃fun s => ⌜s.1 = states ∧  nextOfLt states ∧ s.2.1 = captures ∧ cValid captures⌝⦄
-      Code.c_bounded hir min max greedy possessive
-      ⦃post⟨fun r s => ⌜tRefNextOfLt states r s.1 ∧ cMemAndValid captures s.2.1⌝, fun _ => ⌜True⌝⟩⦄ := by
-  mintro _
-  unfold Code.c_bounded
-  split
-  mspec c_exactly_spec
-  split
-  case isTrue.post.success.isTrue =>
-    split
-    · mspec c_possessive_le_lift_spec
-      inst_mvars
-      case post.success => simp; intros; grind
-      all_goals simp_all
-    · simp_all
-  case isTrue.post.success.isFalse =>
-      mspec add_empty_lift'_spec
-      inst_mvars
-      case post.success =>
-        mspec c_bounded_fold_spec
-        inst_mvars
-        case post.success =>
-          mspec patch_lift_spec
-          · inst_mvars
-            simp_all; grind; grind; all_goals simp_all
-          · simp
-            grind
-        grind; grind; grind; all_goals simp_all
-      all_goals simp_all
-  case isFalse =>
-    mspec c_empty_lift_spec
-    inst_mvars
-    case post.success => simp; intros; grind
-    all_goals simp_all
-termination_by sizeOf hir + sizeOf min + sizeOf (max - min) + 1
-
-@[spec] theorem c_lookaround_spec (look : Lookaround) (states : Array Unchecked.State)
-  (captures : Array NFA.Capture)
-    : ⦃fun s => ⌜s.1 = states ∧ nextOfLt states ∧ s.2.1 = captures ∧ cValid captures⌝⦄
-      Code.c_lookaround look
-      ⦃post⟨fun r s => ⌜tRefNextOfLt states r s.1 ∧ cMemAndValid captures s.2.1⌝, fun _ => ⌜True⌝⟩⦄ := by
-  mintro _
-  unfold Code.c_lookaround
-  split
-  case h_1 | h_2 =>
-    mspec c_spec
-    mspec
-    inst_mvars
-    all_goals simp_all <;> grind
-  case h_3 | h_4 =>
-    mspec add_next_char_lift_spec
-    inst_mvars
-    case post.success =>
-      mspec c_spec
-      inst_mvars
-      case post.success =>
-        mspec
-        inst_mvars
-        case post.success => simp; intros; grind
-        all_goals simp_all <;> grind
-      all_goals simp_all
-    all_goals simp_all
-termination_by sizeOf look
-
-@[spec] theorem c_repetition_spec (rep : Repetition) (states : Array Unchecked.State)
-  (captures : Array NFA.Capture)
-    : ⦃fun s => ⌜s.1 = states ∧ nextOfLt states ∧ s.2.1 = captures ∧ cValid captures⌝⦄
-      Code.c_repetition rep
-      ⦃post⟨fun r s => ⌜tRefNextOfLt states r s.1 ∧ cMemAndValid captures s.2.1⌝, fun _ => ⌜True⌝⟩⦄ := by
-  mintro _
-  unfold Code.c_repetition
-  split
-  case h_1 | h_2 =>
-    mspec
-    inst_mvars
-    case post.success =>
-      mspec c_spec
-      inst_mvars
-      case post.success =>
-        mspec
-        inst_mvars
-        case post.success => simp; intros; grind
-        grind; grind; all_goals simp_all
-      all_goals simp_all
-    all_goals simp_all
-  case h_3 =>
-    split
-    · mspec
-      inst_mvars
-      case post.success =>
-        mspec c_spec
-        inst_mvars
-        case post.success =>
-          mspec
-          inst_mvars
-          case post.success => simp; intros; grind
-          grind; grind; grind; all_goals simp_all
-        all_goals simp_all
-      all_goals simp_all
-    · mspec c_at_least_spec
-  case h_4 =>
-    split
-    mspec c_bounded_spec
-    inst_mvars
-    intros
-    mvcgen <;> simp_all
-termination_by sizeOf rep
-
 @[spec] theorem c_cap_spec (hir : Syntax.Capture) (states : Array Unchecked.State)
   (captures : Array NFA.Capture)
-    : ⦃fun s => ⌜s.1 = states ∧  nextOfLt states ∧ s.2.1 = captures ∧ cValid captures⌝⦄
+    : ⦃fun s => ⌜s.1 = states ∧  NextOfLt states ∧ s.2.1 = captures ∧ cValid captures⌝⦄
       Code.c_cap hir
       ⦃post⟨fun r s => ⌜tRefNextOfLt states r s.1 ∧ cMemAndValid captures s.2.1⌝, fun _ => ⌜True⌝⟩⦄ := by
   mintro _
@@ -1231,16 +1272,16 @@ termination_by sizeOf rep
       case post.success =>
         mspec patch_lift_spec
         inst_mvars
-        case post.success =>
-          simp; intros; and_intros; grind; grind; grind; grind; grind; grind; grind; simp_all
-        simp_all; grind; grind; all_goals simp_all
-      simp_all; grind; grind; all_goals simp_all
-    all_goals simp_all <;> grind
-  all_goals simp_all
+        case post.success => mvcgen with grind [= cValid, = cMemAndValid]
+        all_goals grind
+      all_goals grind
+    simp_all
+    all_goals grind [= cMemAndValid]
+  all_goals grind
 termination_by sizeOf hir
 
 @[spec] theorem c_spec (hir : Hir) (states : Array Unchecked.State) (captures : Array NFA.Capture)
-    : ⦃fun s => ⌜s.1 = states ∧  nextOfLt states ∧ s.2.1 = captures ∧ cValid captures⌝⦄
+    : ⦃fun s => ⌜s.1 = states ∧  NextOfLt states ∧ s.2.1 = captures ∧ cValid captures⌝⦄
       Code.c hir
       ⦃post⟨fun r s => ⌜tRefNextOfLt states r s.1 ∧ cMemAndValid captures s.2.1⌝, fun _ => ⌜True⌝⟩⦄ := by
   have : sizeOf hir.kind < sizeOf hir := Hir.sizeOfKindOfHir hir
@@ -1248,18 +1289,18 @@ termination_by sizeOf hir
   unfold Code.c
   split
   · mspec c_empty_lift_spec
-    inst_mvars; all_goals simp_all
+    inst_mvars; grind; grind; mvcgen with grind
   · mspec c_literal_lift_spec
-    inst_mvars; all_goals simp_all
+    inst_mvars; grind; grind; mvcgen with grind
   · mspec c_unicode_class_lift_spec
-    inst_mvars; all_goals simp_all
+    inst_mvars; grind; grind; mvcgen with grind
   · mspec c_look_lift_spec
-    inst_mvars; all_goals simp_all
+    inst_mvars; grind; grind; mvcgen with grind
   · expose_names
     have : sizeOf look < sizeOf hir.kind := by simp [heq]
     mspec c_lookaround_spec
   · mspec c_back_ref_lift_spec
-    inst_mvars; all_goals simp_all
+    inst_mvars; grind; grind; mvcgen with grind
   · expose_names
     have : sizeOf rep < sizeOf hir.kind := by simp [heq]
     mspec c_repetition_spec
@@ -1269,7 +1310,7 @@ termination_by sizeOf hir
   · expose_names
     have : sizeOf items < sizeOf hir.kind := by simp [heq]
     mspec c_concat_spec
-    inst_mvars; all_goals simp_all
+    grind
   · expose_names
     have : sizeOf sub < sizeOf hir.kind := by simp [heq]
     mspec c_alt_iter_spec
@@ -1280,21 +1321,15 @@ end
 @[spec] theorem c_init_spec (anchored : Bool)
     : ⦃fun s => ⌜s.1.size = 0 ∧ s.2.1.size = 0⌝⦄
       Code.init anchored
-      ⦃post⟨fun r s => ⌜tRefLt r s.1 ∧ nextOfLt s.1 ∧ cValid s.2.1⌝, fun _ => ⌜True⌝⟩⦄ := by
+      ⦃post⟨fun r s => ⌜tRefLt r s.1 ∧ NextOfLt s.1 ∧ cValid s.2.1⌝, fun _ => ⌜True⌝⟩⦄ := by
   mintro _
-  unfold Code.init
-  split
-  · mspec c_empty_lift_spec
-    inst_mvars
-    all_goals simp_all
-  · mspec c_repetition_spec
-    inst_mvars
-    all_goals simp_all
+  mvcgen [Code.init] with exact #[]
+  all_goals grind
 
 @[spec] theorem c_compile_spec (anchored : Bool) (hir : Hir)
     : ⦃fun s => ⌜s.1.size = 0 ∧ s.2.1.size = 0⌝⦄
       Code.compile anchored hir
-      ⦃post⟨fun _ s => ⌜nextOfLt s.1 ∧ cValid s.2.1⌝, fun _ => ⌜True⌝⟩⦄ := by
+      ⦃post⟨fun _ s => ⌜NextOfLt s.1 ∧ cValid s.2.1⌝, fun _ => ⌜True⌝⟩⦄ := by
   mintro _
   unfold Code.compile
   mspec c_init_spec
@@ -1307,24 +1342,24 @@ end
       mspec patch_lift_spec
       inst_mvars
       case post.success =>
-        mspec patch_lift_spec
-        inst_mvars
-        case post.success => simp; intros; grind
-        simp_all; grind; grind; all_goals simp_all
-      simp_all; grind; grind; all_goals simp_all
-    all_goals simp_all
-  all_goals simp_all
+        mvcgen [patch_lift_spec]
+        and_intros; rfl
+        apply NextOfLt.mk
+        all_goals (try rfl) <;> grind
+      all_goals grind
+    all_goals grind
+  all_goals grind
 
 theorem compile_nextOf_lt {anchored : Bool} {expr : Hir}
   (h : Code.compile anchored expr (#[], #[], #[]) = EStateM.Result.ok () (states, captures, groups))
-    : nextOfLt states := by
+    : NextOfLt states := by
   have heq := c_compile_spec anchored expr (#[], #[], #[])
   simp [wp] at heq
   split at heq <;> simp_all
 
 theorem compile_captures_valid {anchored : Bool} {expr : Hir}
   (h : Code.compile anchored expr (#[], #[], #[]) = EStateM.Result.ok () (states, captures, groups))
-    : Capture.valid captures := by
+    : Capture.Valid captures := by
   have heq := c_compile_spec anchored expr (#[], #[], #[])
   simp [wp] at heq
-  split at heq <;> simp_all
+  split at heq <;> grind [= cValid]
