Regex/Compiler/Patch.lean
@@ -44,8 +44,8 @@ def patch («from» «to» : Unchecked.StateID) : PatchM Unit := do
       set (states.set «from» (Unchecked.State.BackRef b f «to»))
     | .ByteRange t =>
         set (states.set «from» (Unchecked.State.ByteRange {t with «next» := «to»}) h)
-    | .Capture role _ pattern_id group_index slot isValid =>
-        set (states.set «from» (Unchecked.State.Capture role «to» pattern_id group_index slot isValid))
+    | .Capture role _ pattern_id group_index =>
+        set (states.set «from» (Unchecked.State.Capture role «to» pattern_id group_index))
     | .BinaryUnion alt1 alt2 =>
         if alt1 = 0
         then set (states.set «from» (Unchecked.State.BinaryUnion «to» alt2) h)
@@ -64,59 +64,73 @@ end Code
 
 namespace Lemmas
 
-theorem all_set_next_of_lt (n : Unchecked.StateID) (s : Unchecked.State)
+@[grind] theorem all_set_next_of_lt (n : Unchecked.StateID) (s : Unchecked.State)
   (states : Array Unchecked.State)
   (h : n < states.size) (hn : Unchecked.State.nextOf s < states.size)
   (hlt : ∀ (i : Nat) _, states[i].nextOf < states.size)
     : ∀ (i : Nat) (hi : i < states.size), (((states.set n s h)[i]'(by grind)).nextOf < states.size) := by
   grind
 
-theorem eat_lt («from» s : Nat) (n : Unchecked.StateID) (m : Unchecked.EatMode)
-  (states : Array Unchecked.State) (h : «from» < states.size)
-  (hmode : Unchecked.EatMode.nextOf m = s)
-  (hm : states[«from»]'h = Unchecked.State.Eat m n)
-  (hlt : states[«from»].nextOf < states.size)
-    : s < states.size ∧ n < states.size := by
-  rw [hm] at hlt
-  simp [Unchecked.EatMode.nextOf] at hmode
-  unfold Unchecked.State.nextOf at hlt
-  split at hlt <;> try simp_all [Nat.max_lt]
+private theorem maxD_of_union_lt («from» : Nat) (s : Array Unchecked.State) (alternates : Array Unchecked.StateID)
+  (h1 : «from» < s.size) (h3 : NextOfLt s)
+  (hm : s[«from»] = Unchecked.State.Union alternates)
+    : List.maxD 0 alternates.toList < s.size := by
+  have h3 := NextOfLt.forall h3
+  have hn := h3 «from» h1
+  rw [hm] at hn
+  unfold  Unchecked.State.nextOf at hn
+  split at hn
+  all_goals grind
 
-theorem change_frame_step_lt («from» : Nat) (f t : Unchecked.StateID)
-  (states : Array Unchecked.State) (h : «from» < states.size)
-  (hm : states[«from»]'h = Unchecked.State.ChangeFrameStep f t)
-  (hlt : states[«from»].nextOf < states.size)
-    : f < states.size ∧ t < states.size := by
-  rw [hm] at hlt
-  unfold Unchecked.State.nextOf at hlt
-  grind
+private theorem maxD_of_union_reverse_lt («from» : Nat) (s : Array Unchecked.State) (alternates : Array Unchecked.StateID)
+  (h1 : «from» < s.size) (h3 : NextOfLt s)
+  (hm : s[«from»] = Unchecked.State.UnionReverse alternates)
+    : List.maxD 0 alternates.toList < s.size := by
+  have h3 := NextOfLt.forall h3
+  have hn := h3 «from» h1
+  rw [hm] at hn
+  unfold  Unchecked.State.nextOf at hn
+  split at hn
+  all_goals grind
 
-theorem binary_union_lt («from» : Nat) (alt1 alt2 : Unchecked.StateID)
-  (states : Array Unchecked.State) (h : «from» < states.size)
-  (hm : states[«from»]'h = Unchecked.State.BinaryUnion alt1 alt2)
-  (hlt : states[«from»].nextOf < states.size)
-    : alt1 < states.size ∧ alt2 < states.size := by
-  rw [hm] at hlt
-  unfold Unchecked.State.nextOf at hlt
-  grind
+@[grind] theorem nextOfLt_of_union («from» to : Nat) (s : Array Unchecked.State) (alternates : Array Unchecked.StateID)
+  (h1 : «from» < s.size) (h2 : to < s.size) (h3 : NextOfLt s)
+  (hm : s[«from»] = Unchecked.State.Union alternates)
+    : NextOfLt (s.set «from» (Unchecked.State.Union (alternates.push to)) h1) := by
+  apply NextOfLt.mk
+  intros i _
+  by_cases hi : i = «from»
+  · unfold Unchecked.State.nextOf
+    split
+    case h_12 =>
+      expose_names
+      have : alternates.toList ++ [to] = alts.toList := by grind
+      have : List.maxD 0 alts.toList < s.size := by
+        rw [← this]
+        exact List.maxD_of_append_lt (maxD_of_union_lt «from» s alternates h1 h3 hm) (by grind)
+      grind
+    all_goals grind
+  · have := NextOfLt.forall h3
+    grind
 
-theorem union_lt («from» to : Nat) (alternates : Array Unchecked.StateID)
-  (states : Array Unchecked.State) (h : «from» < states.size)
-  (ht : to < states.size) (hm : states[«from»]'h = Unchecked.State.Union alternates)
-  (hlt : states[«from»].nextOf < states.size)
-    : List.maxD 0 (alternates.toList ++ [to]) < states.size := by
-  rw [hm] at hlt
-  simp +zetaDelta [Unchecked.State.nextOf] at hlt
-  exact List.maxD_of_append_lt hlt ht
-
-theorem union_reverse_lt («from» to : Nat) (alternates : Array Unchecked.StateID)
-  (states : Array Unchecked.State) (h : «from» < states.size)
-  (ht : to < states.size)
-  (hm : states[«from»]'h = Unchecked.State.UnionReverse alternates)
-  (hlt : states[«from»].nextOf < states.size)
-    : List.maxD 0 (alternates.toList ++ [to]) < states.size := by
-  rw [hm] at hlt
-  simp +zetaDelta [Unchecked.State.nextOf] at hlt
-  exact List.maxD_of_append_lt hlt ht
+@[grind] theorem nextOfLt_of_union_reverse («from» to : Nat) (s : Array Unchecked.State) (alternates : Array Unchecked.StateID)
+  (h1 : «from» < s.size) (h2 : to < s.size) (h3 : NextOfLt s)
+  (hm : s[«from»] = Unchecked.State.UnionReverse alternates)
+    : NextOfLt (s.set «from» (Unchecked.State.UnionReverse (alternates.push to)) h1) := by
+  apply NextOfLt.mk
+  intros i _
+  by_cases hi : i = «from»
+  · unfold Unchecked.State.nextOf
+    split
+    case h_13 =>
+      expose_names
+      have : alternates.toList ++ [to] = alts.toList := by grind
+      have : List.maxD 0 alts.toList < s.size := by
+        rw [← this]
+        exact List.maxD_of_append_lt (maxD_of_union_reverse_lt «from» s alternates h1 h3 hm) (by grind)
+      grind
+    all_goals grind
+  · have := NextOfLt.forall h3
+    grind
 
 end Lemmas
