Regex/NFA/Lemmas.lean
@@ -7,144 +7,47 @@ import Regex.NFA.Basic
 
 namespace NFA
 
-theorem SlotsValidOfRangeMap (slots : Array Capture.SlotGroup)
-  (h : (List.range slots.size).map (fun i => (i, i.div 2)) = slots.toList)
-    : Slots.Valid slots := by
-  simp
-  and_intros
-  · intros
-    expose_names
-    have hMem (a : Capture.SlotGroup) (h : a ∈ (List.range slots.size).map (fun i => (i, i.div 2)))
-        : a.2 = a.1.div 2 := by
-      grind
-    have := hMem (a, b) (by grind)
-    simp_all
-    rw [Nat.mul_comm]
-    have := @Nat.div_add_mod a 2
-    rw [h_2] at this
-    exact id (Eq.symm this)
-  · intros
-    expose_names
-    have hMem (a : Capture.SlotGroup) (h : a ∈ (List.range slots.size).map (fun i => (i, i.div 2)))
-        : a.2 = a.1.div 2 := by
-      grind
-    have := hMem (a, b) (by grind)
-    simp_all
-    rw [Nat.mul_comm]
-    have := @Nat.div_add_mod a 2
-    rw [h_2] at this
-    exact id (Eq.symm this)
-  · intros
-    expose_names
-    exact ⟨a - 1, ⟨b, by
+@[grind] theorem valid_sorted_of_valid (captures : Array NFA.Capture) (h : NFA.Capture.Valid captures)
+    : NFA.Capture.Valid (captures.mergeSort (fun a b => decide (a ≤ b))) := by
+  apply NFA.Capture.Valid.mk
+  have := NFA.Capture.Valid.forall h
+  simp_all
+
+@[grind] theorem valid_unique_of_valid (captures : Array NFA.Capture) (h : NFA.Capture.Valid captures)
+    : NFA.Capture.Valid (captures.unique) := by
+  apply NFA.Capture.Valid.mk
+  have := NFA.Capture.Valid.forall h
+  simp_all
+
+theorem CapturesValidOfRangeMap (captures : Array NFA.Capture)
+  (h : (List.range captures.size).map (fun i =>
+          if i % 2 = 0 then ⟨Capture.Role.Start, i.div 2⟩ else ⟨Capture.Role.End, i.div 2⟩)
+        = captures.toList)
+    : NFA.Capture.Valid captures := by
+  apply NFA.Capture.Valid.mk
+  generalize hf : (fun (i : Nat) => ((if i % 2 = 0 then ⟨Capture.Role.Start, i.div 2⟩
+                                else ⟨Capture.Role.End, i.div 2⟩) : NFA.Capture)) = f at h
+  intro ⟨a, _⟩
+  exact ⟨⟨Capture.Role.Start, a.group⟩, by
     and_intros
-    · have : (a, b) ∈ (List.range slots.size).map (fun i => (i, i.div 2)) := by grind
-      have h : b = (a - 1).div 2 := by
-        rw [h_2]
-        exact Eq.symm (@Nat.div_eq_of_eq_mul_left 2 (b * 2) b (by grind) rfl)
-      have hMem (a : Capture.SlotGroup) (h : a.1 < slots.size ∧ a.2 = a.1.div 2)
-          : a ∈ (List.range slots.size).map (fun i => (i, i.div 2)) := by
-        grind
-      have := hMem (a - 1, b) (And.intro (by grind) h)
-      grind
+    · have h : a ∈ List.map f (List.range captures.size) := by grind
+      have ⟨i, ⟨h1, h2⟩⟩ : ∃ i, i ∈ (List.range captures.size) ∧ f i = a := List.mem_map.mp h
+      rw [← hf] at h2
+      simp at h2
+      split at h2
+      · grind
+      · have h : i % 2 = 1 := by grind
+        have : f (i - 1) ∈ List.map f (List.range captures.size) := by grind
+        have : f (i - 1) ∈ captures := by grind
+        have : f (i - 1) = { role := Capture.Role.Start, group := a.group } := by
+          rw [←hf]
+          simp
+          split
+          · simp
+            have : a.group = i.div 2 := by grind
+            rw [this, ←h]
+            exact Nat.div_eq_sub_mod_div.symm
+          · grind
+        simp_all
     · rfl
-    · grind⟩⟩
-
-instance instLEProdNat : LE Capture.SlotGroup where le := Prod.Lex (· < ·) (· ≤ ·)
-instance instLTProdNat : LT Capture.SlotGroup where lt := Prod.Lex (· < ·) (· < ·)
-
-private theorem mem_toSlots_capture_exists (captures : Array NFA.Capture) (slots : Array Capture.SlotGroup)
-  (h : slots = NFA.Capture.toSlots captures)
-    : ∀ slot ∈ slots, ∃ capture : NFA.Capture, capture ∈ captures ∧ NFA.Capture.toSlots.f capture = slot := by
-  unfold NFA.Capture.toSlots at h
-  simp at h
-  generalize hf : (Array.map NFA.Capture.toSlots.f captures) = filtered at h
-  generalize hs : (filtered.mergeSort NFA.Capture.toSlots.le) = sorted at h
-  intro slot hSlot
-  rw [h] at hSlot
-  have hMemSorted := (Array.mem_unique sorted).mp hSlot
-  rw [← hs] at hMemSorted
-  have hMemFiltered := (Array.mem_mergeSort filtered NFA.Capture.toSlots.le).mp hMemSorted
-  rw [← hf] at hMemFiltered
-  have ⟨state, ⟨hmem, heq⟩⟩ := Array.mem_map.mp hMemFiltered
-  exact ⟨state, by simp [*]⟩
-
-private theorem mem_toSlots_slot_exists (captures : Array NFA.Capture) (slots : Array Capture.SlotGroup)
-  (h : slots = NFA.Capture.toSlots captures)
-    : ∀ capture ∈ captures, (∃ slot ∈ slots, NFA.Capture.toSlots.f capture = slot) := by
-  unfold NFA.Capture.toSlots at h
-  simp at h
-  generalize hf : (Array.map NFA.Capture.toSlots.f captures) = filtered at h
-  generalize hs : (filtered.mergeSort NFA.Capture.toSlots.le) = sorted at h
-  intro capture hCapture
-  let slot := NFA.Capture.toSlots.f capture
-  let hSlot : slot = NFA.Capture.toSlots.f capture := by simp +zetaDelta
-  exact ⟨slot, by
-    have hMemMap := (@Array.mem_map NFA.Capture Capture.SlotGroup slot NFA.Capture.toSlots.f captures).mpr
-                        ⟨capture, And.intro hCapture rfl⟩
-    rw [hf] at hMemMap
-    have hMemSorted := (Array.mem_mergeSort filtered NFA.Capture.toSlots.le).mpr hMemMap
-    rw [hs] at hMemSorted
-    have hMemUnique := (Array.mem_unique sorted).mpr hMemSorted
-    rw [← h] at hMemUnique
-    simp_all⟩
-
-private theorem slotsAreValid_of_slot_mod_eq_0
-  (captures : Array NFA.Capture) (slots : Array Capture.SlotGroup)
-  (hmem : ∀ (slot : Capture.SlotGroup), slot ∈ slots
-          → ∃ capture, capture ∈ captures ∧ NFA.Capture.toSlots.f capture = slot)
-    : ∀ (slot : { slot // slot ∈ slots ∧ slot.fst % 2 = 0 }), slot.val.fst = slot.val.snd * 2 := by
-  intro ⟨s, hs⟩
-  have ⟨capture, hi⟩ := hmem s hs.left
-  unfold NFA.Capture.toSlots.f at hi
-  have hIsValid := capture.isValid
-  simp at hIsValid
-  split at hIsValid
-  · grind
-  · have : s.fst % 2 = 1 := by grind
-    have : s.fst % 2 = 0 := by grind
-    simp_all
-
-private theorem slotsAreValid_of_slot_mod_eq_1
-  (captures : Array NFA.Capture) (slots : Array Capture.SlotGroup)
-  (hmem : ∀ (slot : Capture.SlotGroup), slot ∈ slots
-          → ∃ capture, capture ∈ captures ∧ NFA.Capture.toSlots.f capture = slot)
-    : ∀ (slot : { slot // slot ∈ slots ∧ slot.fst % 2 = 1 }), slot.val.fst = slot.val.snd * 2 + 1 := by
-  intro ⟨s, hs⟩
-  have ⟨capture, hi⟩ := hmem s hs.left
-  unfold NFA.Capture.toSlots.f at hi
-  have hIsValid := capture.isValid
-  simp at hIsValid
-  split at hIsValid <;> grind
-
-private theorem slotsAreValid_if_exists
-  (captures : Array NFA.Capture) (h : NFA.Capture.valid captures)
-  (slots : Array Capture.SlotGroup) (heq : NFA.Capture.toSlots captures = slots)
-  (hmem : ∀ (slot : Capture.SlotGroup), slot ∈ slots
-          → ∃ capture, capture ∈ captures ∧ NFA.Capture.toSlots.f capture = slot)
-    : ∀ (slot : { slot // slot ∈ slots ∧ slot.fst = slot.snd * 2 + 1 }),
-      ∃ slot', slot' ∈ slots ∧ slot.val.snd = slot'.snd ∧ slot'.fst = slot'.snd * 2 := by
-  intro ⟨s, hs⟩
-  have ⟨capture, hCapture⟩ := hmem s hs.left
-  unfold NFA.Capture.valid at h
-  unfold NFA.Capture.toSlots.f at hCapture
-  have hIsValid := capture.isValid
-  simp at hIsValid
-  split at hIsValid; · grind
-  have ⟨capture', hCapture'⟩ := h.right.right ⟨capture, by simp_all⟩
-  have ⟨s', hs'⟩ := mem_toSlots_slot_exists captures slots heq.symm capture' hCapture'.left
-  exact ⟨s', by
-    and_intros
-    simp_all
-    all_goals simp [Capture.toSlots.f] at hs' <;> simp_all <;> grind⟩
-
-theorem toSlots_valid (captures : Array NFA.Capture)
-  (h : NFA.Capture.valid captures)
-    : Slots.Valid (NFA.Capture.toSlots captures) := by
-  generalize hs : NFA.Capture.toSlots captures = slots
-  unfold Slots.Valid
-  have hmem := mem_toSlots_capture_exists captures slots hs.symm
-  and_intros
-  · exact slotsAreValid_of_slot_mod_eq_0 captures slots hmem
-  · exact slotsAreValid_of_slot_mod_eq_1 captures slots hmem
-  · exact slotsAreValid_if_exists captures h slots hs hmem
+    · rfl⟩
