Regex/Notation.lean
@@ -69,13 +69,20 @@ private def mkTermOfLook (l : NFA.Look) : Term :=
 instance : Quote NFA.Look where
   quote := mkTermOfLook
 
-private def mkTermOfRole (l : NFA.Capture.Role) : Term :=
-  match l with
+private def mkTermOfRole (r : NFA.Capture.Role) : Term :=
+  match r with
   | .Start => Syntax.mkApp (mkCIdent ``NFA.Capture.Role.Start) #[]
   | .End => Syntax.mkApp (mkCIdent ``NFA.Capture.Role.End) #[]
 
 instance : Quote NFA.Capture.Role where
   quote := mkTermOfRole
+
+private def mkTermOfCapture (c : NFA.Capture) : Term :=
+  Syntax.mkApp (mkCIdent ``NFA.Capture.mk)
+    #[Quote.quote c.role, Quote.quote c.group]
+
+instance : Quote NFA.Capture where
+  quote := mkTermOfCapture
 
 private def mkTermOfEatMode (m : NFA.Checked.EatMode n) : Term :=
   match m with
@@ -113,9 +120,9 @@ private def mkTermOfState (s : NFA.Checked.State n) : Term :=
       Syntax.mkApp (mkCIdent ``NFA.Checked.State.UnionReverse) #[Quote.quote alts]
   | .BinaryUnion alt1 alt2 =>
       Syntax.mkApp (mkCIdent ``NFA.Checked.State.BinaryUnion) #[Quote.quote alt1, Quote.quote alt2]
-  | .Capture next r id g s _ =>
+  | .Capture next r id g =>
       Syntax.mkApp (mkCIdent ``NFA.Checked.State.Capture)
-        #[Quote.quote next, Quote.quote r, toNumLit id, toNumLit g, toNumLit s, (mkCIdent ``rfl)]
+        #[Quote.quote next, Quote.quote r, toNumLit id, toNumLit g]
   | .Match id =>
       Syntax.mkApp (mkCIdent ``NFA.Checked.State.Match) #[toNumLit id]
 
@@ -125,17 +132,17 @@ instance : Quote (NFA.Checked.State n) where
 private def mkTermIsEq (n : Nat) : Term :=
   Syntax.mkApp (mkCIdent ``Eq.refl) #[toNumLit n]
 
-private def mkTermSlotsValid (slots : Term) : Term :=
-  Syntax.mkApp (mkCIdent ``NFA.SlotsValidOfRangeMap) #[slots,
-      Syntax.mkApp (mkCIdent ``Eq.refl) #[Syntax.mkApp (mkCIdent ``Array.toList) #[slots]]]
+private def mkTermCapturesValid (captures : Term) : Term :=
+  Syntax.mkApp (mkCIdent ``NFA.CapturesValidOfRangeMap) #[captures,
+      Syntax.mkApp (mkCIdent ``rfl) #[]]
 
 private def mkTermOfNfa (nfa : NFA.Checked.NFA) : Term :=
   let states : Term := Quote.quote nfa.states
   let groups : Term := Quote.quote nfa.groups
-  let slots : Term := Quote.quote nfa.slots
+  let captures : Term := Quote.quote nfa.captures
   let flag : Term := Quote.quote nfa.unanchored_prefix_in_backtrack
-  Syntax.mkApp (mkCIdent `NFA.Checked.NFA.mk) #[toNumLit nfa.n, states, groups, slots, flag,
-    mkTermIsEq nfa.n, mkTermSlotsValid slots]
+  Syntax.mkApp (mkCIdent `NFA.Checked.NFA.mk) #[toNumLit nfa.n, states, groups, captures, flag,
+    mkTermIsEq nfa.n, mkTermCapturesValid captures]
 
 private def mkTermOfRegex (re : Regex) : Term :=
   Syntax.mkApp (mkCIdent `Regex.mk) #[mkTermOfNfa re.nfa]
